WiP: restoring the ActualOwnership implementation

fairness/actual_resources.v
@@ -15,329 +15,6 @@ Section actual_ownership.
   Notation "tid ↦m ρ" := (frag_mapping_is {[ tid := {[ ρ ]} ]}) (at level 33).
   Notation "ρ ↦F f" := (frag_fuel_is {[ ρ := f ]}) (at level 33).
 
-  Global Instance ActualOwnershipPartialPre:
-    @PartialModelPredicatesPre _ _ _ Σ M. 
-  Proof.
-    refine {|
-        partial_model_is := frag_model_is;
-        partial_free_roles_are := frag_free_roles_are;
-        partial_fuel_is := frag_fuel_is;
-        partial_mapping_is := frag_mapping_is;
-        partial_msi := model_state_interp;
-      |}.
-    - intros. rewrite /frag_fuel_is.
-      rewrite map_fmap_union. rewrite -gmap_disj_op_union.
-      2: { by apply map_disjoint_fmap. }
-      by rewrite auth_frag_op own_op.
-    - intros. rewrite /frag_free_roles_are.
-      rewrite -gset_disj_union; auto.  
-      by rewrite auth_frag_op own_op.
-    - iApply empty_frag_free_roles. 
-  Defined. 
-
-  Lemma has_fuel_in ζ δ fs n:
-    has_fuels ζ fs -∗ model_state_interp n δ -∗ ⌜ ∀ ρ, ls_mapping δ !! ρ = Some ζ <-> ρ ∈ dom fs ⌝.
-  Proof.
-    unfold model_state_interp, has_fuels, auth_mapping_is, frag_mapping_is.
-    iIntros "[Hζ Hfuels] (%FR&Hafuel&Hamapping &HFR&Hamod&Hfr) %ρ".
-    iCombine "Hamapping Hζ" as "H".
-    iDestruct (own_valid with "H") as %Hval. iPureIntro.
-    apply auth_both_valid_discrete in Hval as [Hval ?].
-    rewrite map_fmap_singleton in Hval.
-    apply singleton_included_exclusive_l in Hval =>//; last by typeclasses eauto.
-    rewrite -> lookup_fmap, leibniz_equiv_iff in Hval.
-    apply fmap_Some_1 in Hval as (R'&HMζ&?). simplify_eq.
-    pose proof (ls_mapping_tmap_corr δ (LM := LM)) as Hmapinv. 
-    rewrite (Hmapinv ρ ζ) HMζ. split.
-    - intros (?&?&?). by simplify_eq.
-    - intros ?. eexists. split; eauto.
-  Qed.
-
-  Lemma has_fuel_fuel ζ δ fs n:
-    has_fuels ζ fs -∗ model_state_interp n δ -∗ 
-    ⌜ ∀ ρ, ρ ∈ dom fs -> ls_fuel δ !! ρ = fs !! ρ ⌝.
-  Proof.
-    unfold has_fuels, model_state_interp, auth_fuel_is.
-    iIntros "[Hζ Hfuels] (%FR&Hafuel&Hamapping&HFR&Hamod)" (ρ Hρ).
-    iDestruct (big_sepS_delete _ _ ρ with "Hfuels") as "[(%f&%Hfs&Hfuel) _]" =>//.
-    iCombine "Hafuel Hfuel" as "H".
-    iDestruct (own_valid with "H") as %Hval. iPureIntro.
-    apply auth_both_valid_discrete in Hval as [Hval ?].
-    rewrite map_fmap_singleton in Hval.
-    apply singleton_included_exclusive_l in Hval =>//; last by typeclasses eauto.
-    rewrite -> lookup_fmap, leibniz_equiv_iff in Hval.
-    apply fmap_Some_1 in Hval as (f'&Hfuelρ&?). simplify_eq.
-    rewrite Hfuelρ Hfs //.
-  Qed.
-
-  Lemma frag_free_roles_fuels_disj: forall n δ fr fs tid,
-        model_state_interp n δ -∗ frag_free_roles_are fr -∗ 
-        has_fuels tid fs (PMPP := ActualOwnershipPartialPre) -∗
-        ⌜ fr ## dom fs⌝. 
-  Proof using. 
-    iIntros (?????) "MSI FREE FUELS". 
-    rewrite /model_state_interp.
-    iAssert (⌜ dom fs ⊆ dom (ls_fuel δ) ⌝)%I as "%INCL2".
-    { iDestruct (has_fuel_fuel with "FUELS MSI") as "%IN".
-      iPureIntro. apply elem_of_subseteq.
-      intros ? DOM. specialize (IN _ DOM).
-      apply elem_of_dom. rewrite IN. by apply elem_of_dom.  }
-    iDestruct "MSI" as (?) "(?&?&FREE'&?&?&%DISJ)".
-    iDestruct (free_roles_inclusion with "FREE' FREE") as "%INCL1".
-    iPureIntro. set_solver. 
-  Qed.
-
-  Definition fuel_apply (fs' F:  gmap (fmrole M) nat) (LR: gset (fmrole M)):
-    gmap (fmrole M) nat :=
-    map_imap
-      (λ (ρ: fmrole M ) (fold : nat),
-       match decide (ρ ∈ dom fs') with
-       | left x => fs' !! ρ
-       | right _ => F !! ρ
-       end) (gset_to_gmap (0%nat) LR).
-
-  Definition update_fuel_resource (δ1: LiveState Λ M) (fs1 fs2: gmap (fmrole M) nat) (s2: M):
-    gmap (fmrole M) nat :=
-
-
-    fuel_apply fs2 (δ1.(ls_fuel (Λ := Λ))) (((dom $ ls_fuel δ1) ∪ dom fs2) ∖ (dom fs1 ∖ dom fs2)).
-
-  Lemma elem_of_frame_excl_map
-        (fs F: gmap (fmrole M) nat)
-        (mf: gmap (fmrole M) (excl nat))
-        (ρ: fmrole M)
-        (f: excl nat):
-    ✓ ((λ f : nat, Excl f) <$> F) ->
-    ((λ f : nat, Excl f) <$> F ≡ ((Excl <$> fs) ⋅? (Some mf))) ->
-    mf !! ρ = Some f ->
-    ρ ∈ dom F ∖ dom fs.
-  Proof.
-    intros Hval Heq Hlk. simpl in Heq.
-    specialize (Heq ρ). rewrite lookup_op Hlk !lookup_fmap in Heq.
-    destruct (decide (ρ ∈ dom F)) as [HF|HF]; last first.
-    { exfalso. apply not_elem_of_dom in HF. rewrite HF //= in Heq.
-      destruct (fs !! ρ) eqn:Hfs; inversion Heq as [A S D G Habs|A Habs];
-        setoid_rewrite -> Hfs in Habs; by compute in Habs. }
-    destruct (decide (ρ ∈ dom fs)) as [Hfs|Hfs].
-    { exfalso. apply elem_of_dom in Hfs as [f' Hlk'].
-      rewrite Hlk' /= in Heq.
-      suffices: Some f = None by eauto.
-      eapply exclusive_Some_l; last first.
-      - specialize (Hval ρ). rewrite -> lookup_fmap, Heq in Hval.
-        apply Hval.
-      - typeclasses eauto. }
-    set_solver.
-  Qed.
-
-  Lemma update_fuel fs fs' F:
-    let LR := (dom F ∪ dom fs') ∖ (dom fs ∖ dom fs') in
-    (fs ≠ ∅) ->
-    (dom fs' ∖ dom fs ∩ dom F = ∅) ->
-    auth_fuel_is F -∗
-    ([∗ map] ρ ↦ f ∈ fs, ρ ↦F f) ==∗
-      auth_fuel_is (fuel_apply fs' F LR) ∗
-      ([∗ map] ρ ↦ f ∈ fs', ρ ↦F f).
-  Proof.
-    iIntros (? Hnotemp Hdisj) "Hafuel Hfuel".
-    rewrite {1}/frag_fuel_is -big_opM_own //.
-    setoid_rewrite map_fmap_singleton.
-    rewrite -big_opM_auth_frag.
-    iCombine "Hafuel Hfuel" as "H".
-    iMod (own_update with "H") as "[A B]"; last first.
-    { iModIntro.
-      destruct (decide (fs' = ∅)) as [Heq|]; last first.
-      -  rewrite {1}/frag_fuel_is -big_opM_own //.
-         iSplitL "A"; done.
-      - rewrite Heq. iSplitL "A"; first done. done. }
-
-    simpl.
-    setoid_rewrite map_fmap_singleton.
-    rewrite -big_opM_auth_frag.
-
-    simpl.
-    apply auth_update.
-
-    apply local_update_discrete.
-
-    intros mf Hval Heq.
-    split.
-    { intros ρ. rewrite /fuel_apply lookup_fmap map_lookup_imap.
-      rewrite lookup_gset_to_gmap.
-      destruct (decide (ρ ∈ LR)).
-      - rewrite option_guard_True //=.
-        destruct (decide (ρ ∈ dom fs')) as [Hd|Hd].
-        + rewrite decide_True //=. apply elem_of_dom in Hd as [? Hsome].
-          rewrite Hsome //.
-        + rewrite decide_False //= -lookup_fmap. apply (Hval ρ).
-      - rewrite option_guard_False //=. }
-
-    intros ρ. rewrite /fuel_apply lookup_fmap map_lookup_imap.
-    rewrite lookup_gset_to_gmap.
-    rewrite -big_opM_fmap big_opM_singletons.
-    rewrite <-big_opM_fmap in Heq. setoid_rewrite big_opM_singletons in Heq.
-    destruct (decide (ρ ∈ LR)).
-    - rewrite option_guard_True //=.
-      destruct (decide (ρ ∈ dom fs')) as [Hd'|Hd'].
-      + rewrite decide_True //=. apply elem_of_dom in Hd' as [? Hsome].
-        rewrite Hsome //= lookup_opM.
-        rewrite lookup_fmap Hsome.
-        destruct mf as [mf|]; simpl; last done.
-        destruct (mf !! ρ) as [f|] eqn:Hlk; rewrite Hlk //.
-
-        assert (ρ ∈ dom F ∖ dom fs).
-        { eauto using elem_of_frame_excl_map. }
-        assert (ρ ∈ dom fs').
-        { apply elem_of_dom. eauto. }
-        set_solver.
-      + rewrite decide_False //= -lookup_fmap.
-        rewrite Heq.
-        destruct (decide (ρ ∈ dom fs)) as [Hd|Hd];
-          first set_solver.
-        pose proof Hd as Hd2. pose proof Hd' as Hd'2.
-        apply not_elem_of_dom in Hd2, Hd'2. rewrite !lookup_opM !lookup_fmap Hd2 Hd'2 //.
-    - rewrite option_guard_False //=.
-      rewrite lookup_opM lookup_fmap.
-      destruct mf as [mf|]; simpl.
-      + destruct (mf !! ρ) as [f|] eqn:Hlk; rewrite Hlk //.
-        * assert (ρ ∈ dom F ∖ dom fs).
-          { eauto using elem_of_frame_excl_map. }
-          set_solver.
-        * assert (Hnotin: ρ ∉ dom fs') by set_solver.
-          apply not_elem_of_dom in Hnotin. rewrite Hnotin //.
-      + assert (Hnotin: ρ ∉ dom fs') by set_solver.
-        apply not_elem_of_dom in Hnotin. rewrite Hnotin //.
-  Qed.
-
-  Lemma update_mapping ζ (R' : gset $ fmrole M) (R: gset (fmrole M)) m :
-    auth_mapping_is m -∗ ζ ↦M R ==∗ auth_mapping_is (<[ ζ := R' ]> m) ∗ ζ ↦M R'.
-  Proof.
-    iIntros "Hamap Hmap".
-    iCombine "Hamap Hmap" as "H".
-    iMod (own_update with "H") as "[A B]"; last first.
-    { iModIntro. iSplitL "A"; iFrame. }
-    rewrite !map_fmap_singleton fmap_insert.
-    eapply auth_update, singleton_local_update_any.
-    intros. by apply exclusive_local_update.
-  Qed.
-
-  Lemma mapping_lookup ζ m R:
-    auth_mapping_is m -∗ ζ ↦M R -∗ ⌜ ζ ∈ dom m ⌝.
-  Proof.
-    unfold auth_mapping_is, frag_mapping_is.
-    iIntros "Ham Hm".
-    iCombine "Ham Hm" as "H".
-    iDestruct (own_valid with "H") as %Hval. iPureIntro.
-    apply auth_both_valid_discrete in Hval as [Hval ?].
-    rewrite map_fmap_singleton in Hval.
-    apply singleton_included_exclusive_l in Hval =>//; last by typeclasses eauto.
-    rewrite -> lookup_fmap, leibniz_equiv_iff in Hval.
-    apply fmap_Some_1 in Hval as (f'&Hfuelρ&?). simplify_eq.
-    apply elem_of_dom. eauto.
-  Qed.
-
-  Lemma update_mapping_new_locale ζ ζ' (R R1 R2 : gset $ fmrole M) m :
-    ζ' ∉ dom m ->
-    auth_mapping_is m -∗
-    ζ ↦M R ==∗
-    auth_mapping_is (<[ ζ' := R2]> (<[ ζ := R1 ]> m)) ∗
-    ζ ↦M R1 ∗ ζ' ↦M R2.
-  Proof.
-    iIntros (Hnotin) "Hamap Hmap".
-    iDestruct (mapping_lookup with "Hamap Hmap") as %Hin.
-    iCombine "Hamap Hmap" as "H".
-    iMod (own_update (A := (authUR (gmapUR _ (exclR (gsetR (RoleO M)))))) _ _ (
-                       ● ((λ f : gset (fmrole M), Excl f) <$> ((<[ ζ := R1 ]> m)))
-                         ⋅ ◯ ((λ f : gset (fmrole M), Excl f) <$> {[ζ := R1]})
-                     ) with "H") as "[A B]".
-    { rewrite !map_fmap_singleton fmap_insert.
-      eapply auth_update. eapply singleton_local_update_any.
-      intros. by apply exclusive_local_update. }
-    iCombine "A B" as "H".
-    iMod (own_update (A := (authUR (gmapUR _ (exclR (gsetR (RoleO M)))))) _ _ (
-                       ● ((λ f : gset (fmrole M), Excl f) <$> (<[ ζ' := R2]> (<[ ζ := R1 ]> m)))
-                         ⋅ ◯ ((λ f : gset (fmrole M), Excl f) <$> {[ζ := R1 ; ζ' := R2]})
-                     ) with "H") as "[A B]"; last first.
-    { iModIntro. iSplitL "A"; first iFrame. rewrite !fmap_insert fmap_empty insert_empty.
-      replace (◯ {[ζ := Excl R1; ζ' := Excl R2]}) with (◯ {[ζ := Excl R1]} ⋅ ◯ {[ζ' := Excl R2]}).
-      - iDestruct "B" as "[A B]". iSplitL "A"; rewrite /frag_mapping_is map_fmap_singleton //.
-      - rewrite -auth_frag_op insert_singleton_op //. rewrite lookup_singleton_ne //. set_solver. }
-    rewrite !map_fmap_singleton fmap_insert !fmap_insert.
-    rewrite (insert_commute _ _ _ (Excl R1) (Excl R2)); last set_solver.
-    eapply auth_update. rewrite fmap_empty. eapply alloc_local_update; eauto.
-    - rewrite lookup_insert_ne; last set_solver. apply not_elem_of_dom. set_solver.
-    - done.
-  Qed.
-
-  Lemma update_mapping_delete ζ (Rrem : gset $ fmrole M) (R: gset (fmrole M)) m :
-    auth_mapping_is m -∗ ζ ↦M R ==∗ auth_mapping_is (<[ ζ := R ∖ Rrem ]> m) ∗ ζ ↦M (R ∖ Rrem).
-  Proof.
-    eauto using update_mapping.
-  Qed.
-
-  Lemma update_mapping_add ζ (Radd : gset $ fmrole M) (R: gset (fmrole M)) m :
-    auth_mapping_is m -∗ ζ ↦M R ==∗ auth_mapping_is (<[ ζ := R ∪ Radd ]> m) ∗ ζ ↦M (R ∪ Radd).
-  Proof.
-    eauto using update_mapping.
-  Qed.
-
-
-  Lemma update_has_fuels ζ fs fs' F m :
-    let LR := (dom F ∪ dom fs') ∖ (dom fs ∖ dom fs') in
-    (fs ≠ ∅) ->
-    (dom fs' ∖ dom fs ∩ dom F = ∅) ->
-    has_fuels ζ fs -∗
-    auth_fuel_is F -∗
-    auth_mapping_is m ==∗
-    auth_fuel_is (fuel_apply fs' F LR) ∗
-    has_fuels ζ fs' ∗
-    auth_mapping_is (<[ ζ := dom fs' ]> m).
-  Proof.
-    iIntros (LR Hfs Hdom) "Hfuels Hafuels Hamapping".
-    rewrite !has_fuels_equiv. iDestruct "Hfuels" as "[Hmapping Hfuels]".    
-    iMod (update_fuel with "Hafuels Hfuels") as "[Hafuels Hfuels]" =>//.
-    iMod (update_mapping with "Hamapping Hmapping") as "[Hamapping Hmapping]".
-    iModIntro.
-    iFrame.
-  Qed.
-
-  Lemma update_has_fuels_no_step ζ fs fs' F m :
-    let LR := (dom F ∪ dom fs') ∖ (dom fs ∖ dom fs') in
-    (fs ≠ ∅) ->
-    (dom fs' ⊆ dom fs) ->
-    has_fuels ζ fs -∗
-    auth_fuel_is F -∗
-    auth_mapping_is m ==∗
-    auth_fuel_is (fuel_apply fs' F LR) ∗
-    has_fuels ζ fs' ∗
-    auth_mapping_is (<[ ζ := dom fs' ]> m).
-  Proof.
-    iIntros (LR Hfs Hdom) "Hfuels Hafuels Hamapping".
-    rewrite !has_fuels_equiv. iDestruct "Hfuels" as "[Hmapping Hfuels]".
-    iMod (update_fuel fs fs' with "Hafuels Hfuels") as "[Hafuels Hfuels]"; [done|set_solver|].
-    iMod (update_mapping with "Hamapping Hmapping") as "[Hamapping Hmapping]".
-    iModIntro. iFrame.
-  Qed.
-
-  Lemma update_has_fuels_no_step_no_change ζ fs fs' F m :
-    let LR := (dom F ∪ dom fs') ∖ (dom fs ∖ dom fs') in
-    (fs ≠ ∅) ->
-    (dom fs' = dom fs) ->
-    has_fuels ζ fs -∗
-    auth_fuel_is F -∗
-    auth_mapping_is m ==∗
-    auth_fuel_is (fuel_apply fs' F LR) ∗
-    has_fuels ζ fs' ∗
-    auth_mapping_is m.
-  Proof.
-    iIntros (LR Hfs Hdom) "Hfuels Hafuels Hamapping".
-    rewrite !has_fuels_equiv. iDestruct "Hfuels" as "[Hmapping Hfuels]".
-    iMod (update_fuel fs fs' with "Hafuels Hfuels") as "[Hafuels Hfuels]" =>//.
-    { rewrite Hdom. set_solver. }
-    iModIntro.
-    iFrame. rewrite Hdom //.
-  Qed.
-
-
 End actual_ownership. 
 
 Section ActualOwnershipImpl.
@@ -347,86 +24,55 @@ Section ActualOwnershipImpl.
   Context {Σ : gFunctors}.
   Context {fG: fairnessGS LM Σ}.
 
-  Lemma tids_smaller_restrict_mapping (c1 c2: cfg Λ) δ1 δ2 (ζ: locale Λ)
-    (Hζs : tids_smaller c1.1 δ1)
-    (DOM12: ls_mapping δ2 ⊆ ls_mapping δ1)
-    (STEP: locale_step c1 (Some ζ) c2)
-    :
-    tids_smaller c2.1 δ2 (M := M).
+  Lemma mim_fuel_helper (fs: gmap (fmrole M) nat) rem ζ
+    (tmap1: gmap (locale Λ) (gset (fmrole M)))
+    map1
+    (Hincl : rem ⊆ dom fs)
+    (Hxdom : ∀ ρ : fmrole M, map1 !! ρ = Some ζ ↔ ρ ∈ dom (S <$> fs))
+    (Hminv1 : maps_inverse_match map1 tmap1):
+  maps_inverse_match
+    (filter (λ '(k, _), k ∈ (dom map1 ∪ dom fs) ∖ rem) map1)
+    (<[ζ:=dom (filter (λ '(k, _), k ∈ dom fs ∖ rem) fs)]> tmap1).
   Proof.
-    unfold tids_smaller; simpl.
-    intros ρ ζ0 Hin.
-    destruct c1, c2.
-    eapply from_locale_step =>//.
-    rewrite /tids_smaller /= in Hζs. eapply Hζs.
-    eapply lookup_weaken; eauto. 
-  Qed.
-
-
-  (* TODO: the info below should be used, as it'll be related to the lemma above *)
-  (* (TMAP2: tmap2 = <[ζ:=dom (filter (λ '(k, _), k ∈ dom fs ∖ rem) fs)]> (tmap1)) *)
-  Lemma tids_dom_restrict_mapping (c1 c2: cfg Λ)
-    (tmap1 tmap2: gmap (locale Λ) (gset (fmrole M))) (ζ: locale Λ)
-    (* (fs: gmap (fmrole M) nat) *)
-    (* rem *)
-
-    (XX: gset (fmrole M))
-    
-    (Hstep : locale_step c1 (Some ζ) c2)
-  (Hlocssmall : ∀ ζ : locale Λ, ζ ∉ locales_of_list c1.1 → tmap1 !! ζ = None)
-  (TMAP2: tmap2 = <[ζ:=XX]> (tmap1))
-    :
-  ∀ ζ0 : locale Λ,
-    ζ0 ∉ locales_of_list c2.1 →
-    (* <[ζ:=dom (filter (λ '(k, _), k ∈ dom fs ∖ rem) fs)]> (ls_tmap δ1) !! ζ0 = *)
-    (tmap2) !! ζ0 = None.
-  Proof.
-    intros ζ0 Hnotin.
-    rewrite TMAP2. 
-    destruct c1, c2. simpl in *. 
-    apply lookup_insert_None; split.
-    + apply Hlocssmall.
-      have Hle := locales_of_list_step_incl _ _ _ _ _ Hstep. simpl.
-      clear -Hnotin Hle. set_solver.
-    + intros <-. 
-      have ? := locales_of_list_step_incl _ _ _ _ _ Hstep. simpl.
-      (* clear Hfueldom Hsamedoms. *)
-      inversion Hstep. simplify_eq.
-      assert (locale_of t1 e1 ∈ locales_of_list (t1 ++ e1 :: t2));
-        last by eauto.
-      apply locales_of_list_from_locale_from.
-      rewrite from_locale_from_Some //. 
-      eapply prefixes_from_spec.
-      eexists _,_. by list_simplifier.
-  Qed.
-  (* TODO: ?? *)
-    (* - rewrite Hnewdom /new_dom. apply elem_of_equiv_empty_L. intros ρ [Hin1 Hin2]%elem_of_intersection. *)
-    (*   assert (ρ ∈ dom (ls_fuel δ1)) *)
-    (*     by set_solver -Hnewdom Hsamedoms Hfueldom. *)
-    (*   set_solver -Hnewdom Hsamedoms Hfueldom. } *)
- 
-
+    intros ρ ζ'. rewrite dom_domain_restrict; last set_solver. split.
+    + intros [Hlk Hin]%map_filter_lookup_Some. destruct (decide (ζ' = ζ)) as [->|Hneq].
+      * rewrite lookup_insert. eexists; split=>//.
+        set_solver.
+      * rewrite lookup_insert_ne //. by eapply Hminv1.
+    + intros Hin. destruct (decide (ζ' = ζ)) as [->|Hneq].
+      * rewrite lookup_insert in Hin. apply map_filter_lookup_Some.
+        destruct Hin as (?&?&?). simplify_eq. split; last set_solver.
+        apply Hxdom. rewrite dom_fmap. set_solver.
+      * rewrite lookup_insert_ne // -Hminv1 in Hin. apply map_filter_lookup_Some; split=>//.
+        apply elem_of_difference; split.
+        ** apply elem_of_dom_2 in Hin. set_solver.
+        ** assert (ρ ∉ dom fs); last set_solver.
+           rewrite dom_fmap_L in Hxdom.
+           intros contra%Hxdom. congruence.
+  Qed. 
 
   Lemma actual_update_no_step_enough_fuel
-  (δ1: LM) rem c1 c2 fs ζ:
+  (δ1: LM) rem
+  (* c1 c2 *)
+  fs ζ:
     (dom fs ≠ ∅) ->
     (live_roles _ δ1) ∩ rem = ∅ →
     rem ⊆ dom fs →
-    locale_step c1 (Some ζ) c2 ->
-    has_fuels_S ζ fs -∗ model_state_interp c1 δ1
+    (* locale_step c1 (Some ζ) c2 -> *)
+    has_fuels_S ζ fs -∗ model_state_interp δ1
     ==∗ ∃ δ2,
-        ⌜
-         labels_match (LM:=LM) (Some ζ) (Silent_step ζ) ∧ 
-          valid_evolution_step (Some ζ) c2 δ1 (Silent_step ζ) δ2 (LM := LM)⌝ ∗
-            has_fuels ζ (fs ⇂ (dom fs ∖ rem)) ∗ model_state_interp c2 δ2.
-  Proof.
-    iIntros "%HnotO %Holdroles %Hincl %Hstep Hf Hmod".
-    destruct c2 as [tp2 σ2].
+        ⌜ lm_ls_trans LM δ1 (Silent_step ζ) δ2 ⌝ ∗
+        has_fuels ζ (fs ⇂ (dom fs ∖ rem)) ∗
+        model_state_interp δ2 ∗
+        ⌜ ls_tmap δ2 (LM := LM) = <[ζ:=dom (filter (λ '(k, _), k ∈ dom fs ∖ rem) fs)]> (ls_tmap δ1 (LM := LM)) ⌝. 
+Proof.
+    iIntros "%HnotO %Holdroles %Hincl Hf Hmod".
+    (* destruct c2 as [tp2 σ2]. *)
     destruct (set_choose_L _ HnotO) as [??].
     iDestruct (has_fuel_in with "Hf Hmod") as %Hxdom; eauto.
     iDestruct (has_fuel_fuel with "Hf Hmod") as "%Hfuel"; eauto.
-    iDestruct (model_state_interp_tids_smaller with "Hmod") as %Hζs.
-    iDestruct "Hmod" as "(%FR & Hfuel & Hamapping & HFR & %Hlocssmall & Hmodel & %HFR)".
+    (* iDestruct (model_state_interp_tids_smaller with "Hmod") as %Hζs. *)
+    iDestruct "Hmod" as "(%FR & Hfuel & Hamapping & HFR & Hmodel & %HFR)".
     unfold has_fuels_S.
     simpl in *.
 
@@ -465,7 +111,7 @@ Section ActualOwnershipImpl.
     { rewrite /fuel_apply Hnewdom.
       intros ρ Hin. apply elem_of_difference; split;
         [apply ls_fuel_dom in Hin; set_solver +Hin|
-          set_solver -Hlocssmall Hnewdom Hsamedoms]. }
+          set_solver -Hnewdom Hsamedoms]. }
     iMod (update_has_fuels_no_step ζ (S <$> fs) (fs ⇂ (dom fs ∖ rem)) with "[Hf] [Hfuel] [Hamapping]") as "(Hafuels&Hfuels&Hamapping)" =>//.
     { rewrite -dom_empty_iff_L. set_solver -Hnewdom Hsamedoms Hfueldom. }
     { rewrite dom_domain_restrict; set_solver -Hnewdom Hsamedoms Hfueldom. }
@@ -483,49 +129,33 @@ Section ActualOwnershipImpl.
     assert (maps_inverse_match new_mapping (<[ζ:=dom (filter (λ '(k, _), k ∈ dom fs ∖ rem) fs)]>
       (ls_tmap δ1 (LM := LM))
            )) as MATCH.
-    { intros ρ ζ'. rewrite /new_mapping dom_domain_restrict; last set_solver +. split.
-      + intros [Hlk Hin]%map_filter_lookup_Some. destruct (decide (ζ' = ζ)) as [->|Hneq].
-        * rewrite lookup_insert. eexists; split=>//.
-          set_solver -Hnewdom Hsamedoms.
-        * rewrite lookup_insert_ne //. by eapply Hminv1.
-      + intros Hin. destruct (decide (ζ' = ζ)) as [->|Hneq].
-        * rewrite lookup_insert in Hin. apply map_filter_lookup_Some.
-          destruct Hin as (?&?&?). simplify_eq. split; last set_solver -Hnewdom Hsamedoms Hfueldom.
-          apply Hxdom. rewrite dom_fmap. set_solver -Hnewdom Hsamedoms Hfueldom.
-        * rewrite lookup_insert_ne // -Hminv1 in Hin. apply map_filter_lookup_Some; split=>//.
-          rewrite /new_dom. apply elem_of_difference; split.
-          ** apply elem_of_dom_2 in Hin. rewrite ls_same_doms in Hin. set_solver -Hnewdom Hsamedoms.
-          ** assert (ρ ∉ dom fs); last set_solver -Hnewdom Hsamedoms.
-             rewrite dom_fmap_L in Hxdom.
-             intros contra%Hxdom. congruence. }
+    { clear -Hxdom Hminv1 Hincl.
+      subst new_mapping new_dom. 
+      rewrite -ls_same_doms. 
+      apply mim_fuel_helper; auto. }
 
-    (* assert (ls_mapping δ2 = new_mapping) as MAP_ALT. *)
-    (* { eapply maps_inverse_match_uniq1. *)
-    (*   - eapply ls_mapping_tmap_corr. *)
-    (*   - rewrite Heqδ2. rewrite (build_LS_ext_spec_tmap (LM := LM)).  *)
-    (*   2: by apply MATCH.  *)
-    (*   - eapply ls_mapping_tmap_corr. *)
-    (*   - eauto.   *)
-
-
-    simpl.
+    simpl. 
     iSplit; last first.
-    { rewrite (dom_fmap_L _ fs). iFrame "Hfuels". iExists FR.
+    { rewrite (dom_fmap_L _ fs). iFrame "Hfuels". 
       (* rewrite /maps_inverse_match //=. *)
+      rewrite /model_state_interp. 
       rewrite build_LS_ext_spec_st build_LS_ext_spec_fuel build_LS_ext_spec_tmap.
       iFrame.
+      iSplitL; [| done]. 
       assert (dom fs ⊆ dom (ls_fuel $ δ1)).
       { intros ρ Hin. setoid_rewrite dom_fmap in Hxdom.
         specialize (Hxdom ρ). rewrite -ls_same_doms. apply elem_of_dom. exists ζ.
         by apply Hxdom. }
+      iExists _. iFrame. 
       iSplit.
       { iApply (auth_fuel_is_proper with "Hafuels"). f_equiv.
         rewrite dom_domain_restrict; last set_solver -Hnewdom Hsamedoms Hfueldom.
         replace (dom fs ∖ (dom fs ∖ rem)) with rem; [set_solver +|].
         rewrite -leibniz_equiv_iff. intros ρ. split; [set_solver -Hnewdom Hsamedoms Hfueldom|].
         intros [? [?|?]%not_elem_of_difference]%elem_of_difference =>//. }
-      iPureIntro. split.
-      - intros. eapply tids_dom_restrict_mapping; eauto. 
+      iPureIntro.
+      (* split. *)
+      (* - intros. eapply tids_dom_restrict_mapping; eauto.  *)
       - rewrite Hnewdom /new_dom. apply elem_of_equiv_empty_L. intros ρ [Hin1 Hin2]%elem_of_intersection.
         assert (ρ ∈ dom (ls_fuel δ1))
                by set_solver -Hnewdom Hsamedoms Hfueldom.
@@ -538,9 +168,8 @@ Section ActualOwnershipImpl.
          admit. }
     
     iPureIntro.
-    do 2 split; first done.
     (* split; [split; [|split; [|split; [|split]]]|] =>//. *)
-    repeat split.
+    repeat split; try done. 
     - eexists. apply Hxdom. by rewrite dom_fmap.
     - unfold fuel_decr. simpl.
       rewrite (build_LS_ext_spec_fuel). 
@@ -587,9 +216,9 @@ Section ActualOwnershipImpl.
       intros ρ Hin. apply elem_of_dom.
       rewrite Hfuel ?dom_fmap // -elem_of_dom dom_fmap //.
     - by rewrite build_LS_ext_spec_st.   
-    - eapply tids_smaller_restrict_mapping; eauto.
-      erewrite build_LS_ext_spec_mapping; [| by eauto].
-      subst new_mapping. apply map_filter_subseteq. 
+    (* - eapply tids_smaller_restrict_mapping; eauto. *)
+    (*   erewrite build_LS_ext_spec_mapping; [| by eauto]. *)
+    (*   subst new_mapping. apply map_filter_subseteq.  *)
   Admitted.
 
   Lemma tids_smaller_fork_step σ1 σ2 δ1 δ2 ζ τ_new
@@ -677,659 +306,659 @@ Section ActualOwnershipImpl.
   Qed.
 
 
-  Lemma actual_update_fork_split R1 R2 tp1 tp2 fs (δ1: LM) ζ τ_new σ1 σ2 (Hdisj: R1 ## R2):
-    fs ≠ ∅ ->
-    R1 ∪ R2 = dom fs ->
-    (* trace_last extr = (tp1, σ1) -> *)
-    locale_step (tp1, σ1) (Some ζ) (tp2, σ2) ->
-    (* (∃ tp1', tp2 = tp1' ++ [efork] ∧ length tp1' = length tp1) -> *)
-    τ_new ∉ dom (ls_tmap δ1 (LM := LM)) ->
-    has_fuels_S ζ fs -∗ model_state_interp (tp1, σ1) δ1 ==∗
-      ∃ δ2, has_fuels τ_new (fs ⇂ R2) ∗ has_fuels ζ (fs ⇂ R1) ∗
-            (partial_mapping_is {[ τ_new := ∅ ]} -∗ frag_mapping_is {[ τ_new := ∅ ]}) ∗
-            model_state_interp (tp2, σ2) δ2
-        ∧ ⌜valid_evolution_step (Some ζ) (tp2, σ2) δ1 (Silent_step ζ) δ2 (LM := LM)⌝.
-  Proof.
-    iIntros (Hnemp Hunioneq Hstep Hnewζ) "Hf Hmod".
-    unfold has_fuels_S.
-    simpl in *.
-    iDestruct (has_fuel_fuel with "Hf Hmod") as %Hfuels.
-    iDestruct (model_state_interp_tids_smaller with "Hmod") as %Hts.
-    iDestruct "Hmod" as (FR) "(Haf&Ham&HFR&%Hsmall&Hamod&%HFR)".
-    pose Hlocincl := locales_of_list_step_incl _ _ _ _ _ Hstep.
-    iMod (update_has_fuels_no_step_no_change ζ (S <$> fs) fs with "Hf Haf Ham") as "(Haf&Hf&Ham)".
-    { intros contra. apply fmap_empty_inv in contra. set_solver. }
-    { rewrite dom_fmap_L //. }
-    iDestruct "Hf" as "(Hf & Hfuels)".
-    iDestruct (frag_mapping_same with "Ham Hf") as %Hmapping.
-    (* assert (Hnewζ: (locale_of tp1 efork) ∉ dom (ls_tmap δ1)). *)
-    (* { apply not_elem_of_dom. apply Hsmall. *)
-    (*   unfold tids_smaller in Hsmall. *)
-    (*   rewrite elem_of_list_fmap. intros ([??]&Hloc&Hin). *)
-    (*   symmetry in Hloc. *)
-    (*   rewrite -> prefixes_from_spec in Hin. *)
-    (*   destruct Hin as (?&t0&?&?). *)
-    (*   simplify_eq. list_simplifier. *)
-    (*   eapply locale_injective=>//. *)
-    (*   apply prefixes_from_spec. *)
-    (*   exists t0, []. split =>//. by list_simplifier. } *)
-    iMod (update_mapping_new_locale ζ τ_new _ R1 R2 with "Ham Hf") as "(Ham&HR1&HR2)"; eauto.
-    assert (Hsamedoms: dom (map_imap
-                                (λ ρ o,
-                                 if decide (ρ ∈ R2) then Some $ τ_new else Some o)
-                                (ls_mapping δ1)) =
-                         dom (map_imap
-                             (λ ρ o,
-                              if decide (ρ ∈ R1 ∪ R2) then Some (o - 1)%nat else Some o)
-                             (ls_fuel δ1))
-           ).
-    { rewrite !map_imap_dom_eq; first by rewrite ls_same_doms.
-      - by intros ρ??; destruct (decide (ρ ∈ R1 ∪ R2)).
-      - by intros ρ??; destruct (decide (ρ ∈ R2)). }
-    assert (Hfueldom: live_roles _ δ1 ⊆ dom (map_imap
-                             (λ ρ o,
-                              if decide (ρ ∈ R1 ∪ R2) then Some (o - 1)%nat else Some o)
-                             (ls_fuel δ1))).
-    { rewrite map_imap_dom_eq; first by apply ls_fuel_dom.
-      - by intros ρ??; destruct (decide (ρ ∈ R1 ∪ R2)). }
+  (* Lemma actual_update_fork_split R1 R2 tp1 tp2 fs (δ1: LM) ζ τ_new σ1 σ2 (Hdisj: R1 ## R2): *)
+  (*   fs ≠ ∅ -> *)
+  (*   R1 ∪ R2 = dom fs -> *)
+  (*   (* trace_last extr = (tp1, σ1) -> *) *)
+  (*   locale_step (tp1, σ1) (Some ζ) (tp2, σ2) -> *)
+  (*   (* (∃ tp1', tp2 = tp1' ++ [efork] ∧ length tp1' = length tp1) -> *) *)
+  (*   τ_new ∉ dom (ls_tmap δ1 (LM := LM)) -> *)
+  (*   has_fuels_S ζ fs -∗ model_state_interp (tp1, σ1) δ1 ==∗ *)
+  (*     ∃ δ2, has_fuels τ_new (fs ⇂ R2) ∗ has_fuels ζ (fs ⇂ R1) ∗ *)
+  (*           (partial_mapping_is {[ τ_new := ∅ ]} -∗ frag_mapping_is {[ τ_new := ∅ ]}) ∗ *)
+  (*           model_state_interp (tp2, σ2) δ2 *)
+  (*       ∧ ⌜valid_evolution_step (Some ζ) (tp2, σ2) δ1 (Silent_step ζ) δ2 (LM := LM)⌝. *)
+  (* Proof. *)
+  (*   iIntros (Hnemp Hunioneq Hstep Hnewζ) "Hf Hmod". *)
+  (*   unfold has_fuels_S. *)
+  (*   simpl in *. *)
+  (*   iDestruct (has_fuel_fuel with "Hf Hmod") as %Hfuels. *)
+  (*   iDestruct (model_state_interp_tids_smaller with "Hmod") as %Hts. *)
+  (*   iDestruct "Hmod" as (FR) "(Haf&Ham&HFR&%Hsmall&Hamod&%HFR)". *)
+  (*   pose Hlocincl := locales_of_list_step_incl _ _ _ _ _ Hstep. *)
+  (*   iMod (update_has_fuels_no_step_no_change ζ (S <$> fs) fs with "Hf Haf Ham") as "(Haf&Hf&Ham)". *)
+  (*   { intros contra. apply fmap_empty_inv in contra. set_solver. } *)
+  (*   { rewrite dom_fmap_L //. } *)
+  (*   iDestruct "Hf" as "(Hf & Hfuels)". *)
+  (*   iDestruct (frag_mapping_same with "Ham Hf") as %Hmapping. *)
+  (*   (* assert (Hnewζ: (locale_of tp1 efork) ∉ dom (ls_tmap δ1)). *) *)
+  (*   (* { apply not_elem_of_dom. apply Hsmall. *) *)
+  (*   (*   unfold tids_smaller in Hsmall. *) *)
+  (*   (*   rewrite elem_of_list_fmap. intros ([??]&Hloc&Hin). *) *)
+  (*   (*   symmetry in Hloc. *) *)
+  (*   (*   rewrite -> prefixes_from_spec in Hin. *) *)
+  (*   (*   destruct Hin as (?&t0&?&?). *) *)
+  (*   (*   simplify_eq. list_simplifier. *) *)
+  (*   (*   eapply locale_injective=>//. *) *)
+  (*   (*   apply prefixes_from_spec. *) *)
+  (*   (*   exists t0, []. split =>//. by list_simplifier. } *) *)
+  (*   iMod (update_mapping_new_locale ζ τ_new _ R1 R2 with "Ham Hf") as "(Ham&HR1&HR2)"; eauto. *)
+  (*   assert (Hsamedoms: dom (map_imap *)
+  (*                               (λ ρ o, *)
+  (*                                if decide (ρ ∈ R2) then Some $ τ_new else Some o) *)
+  (*                               (ls_mapping δ1)) = *)
+  (*                        dom (map_imap *)
+  (*                            (λ ρ o, *)
+  (*                             if decide (ρ ∈ R1 ∪ R2) then Some (o - 1)%nat else Some o) *)
+  (*                            (ls_fuel δ1)) *)
+  (*          ). *)
+  (*   { rewrite !map_imap_dom_eq; first by rewrite ls_same_doms. *)
+  (*     - by intros ρ??; destruct (decide (ρ ∈ R1 ∪ R2)). *)
+  (*     - by intros ρ??; destruct (decide (ρ ∈ R2)). } *)
+  (*   assert (Hfueldom: live_roles _ δ1 ⊆ dom (map_imap *)
+  (*                            (λ ρ o, *)
+  (*                             if decide (ρ ∈ R1 ∪ R2) then Some (o - 1)%nat else Some o) *)
+  (*                            (ls_fuel δ1))). *)
+  (*   { rewrite map_imap_dom_eq; first by apply ls_fuel_dom. *)
+  (*     - by intros ρ??; destruct (decide (ρ ∈ R1 ∪ R2)). } *)
 
-    (* iExists {| *)
-    (*   ls_under := δ1.(ls_under); *)
-    (*   ls_fuel := _; *)
-    (*   ls_fuel_dom := Hfueldom; *)
-    (*   ls_mapping := _; *)
-    (*   ls_same_doms := Hsamedoms; *)
-    (* |}. *)
-    iExists (build_LS_ext (ls_under δ1) _ Hfueldom _ _ _ (LM := LM)).
+  (*   (* iExists {| *) *)
+  (*   (*   ls_under := δ1.(ls_under); *) *)
+  (*   (*   ls_fuel := _; *) *)
+  (*   (*   ls_fuel_dom := Hfueldom; *) *)
+  (*   (*   ls_mapping := _; *) *)
+  (*   (*   ls_same_doms := Hsamedoms; *) *)
+  (*   (* |}. *) *)
+  (*   iExists (build_LS_ext (ls_under δ1) _ Hfueldom _ _ _ (LM := LM)). *)
 
-    iModIntro.
-    assert (Hdomincl: dom fs ⊆ dom (ls_fuel δ1)).
-    { intros ρ' Hin'. rewrite elem_of_dom Hfuels; last first.
-      { rewrite dom_fmap_L //. }
-      rewrite lookup_fmap fmap_is_Some. by apply elem_of_dom. }
-    rewrite -Hunioneq big_sepS_union //. iDestruct "Hfuels" as "[Hf1 Hf2]".
-    iSplitL "Hf2 HR2".
-    { unfold has_fuels.
-      rewrite dom_domain_restrict;
-        [|set_solver -Hsamedoms Hsamedoms Hfueldom Hlocincl Hdomincl].
-      iFrame.
-      iApply (big_sepS_impl with "Hf2"). iIntros "!#" (x Hin) "(%f&%&?)".
-      iExists _; iFrame. iPureIntro. rewrite map_filter_lookup_Some //. }    
-    iSplitL "Hf1 HR1".
-    { unfold has_fuels.
-      rewrite dom_domain_restrict;
-        [|set_solver -Hsamedoms Hsamedoms Hfueldom Hlocincl Hdomincl].
-      iFrame.
-      iApply (big_sepS_impl with "Hf1"). iIntros "!#" (x Hin) "(%f&%&?)".
-      iExists _; iFrame. iPureIntro. rewrite map_filter_lookup_Some //. }
-    iSplitR; [iIntros; by iFrame | ].
+  (*   iModIntro. *)
+  (*   assert (Hdomincl: dom fs ⊆ dom (ls_fuel δ1)). *)
+  (*   { intros ρ' Hin'. rewrite elem_of_dom Hfuels; last first. *)
+  (*     { rewrite dom_fmap_L //. } *)
+  (*     rewrite lookup_fmap fmap_is_Some. by apply elem_of_dom. } *)
+  (*   rewrite -Hunioneq big_sepS_union //. iDestruct "Hfuels" as "[Hf1 Hf2]". *)
+  (*   iSplitL "Hf2 HR2". *)
+  (*   { unfold has_fuels. *)
+  (*     rewrite dom_domain_restrict; *)
+  (*       [|set_solver -Hsamedoms Hsamedoms Hfueldom Hlocincl Hdomincl]. *)
+  (*     iFrame. *)
+  (*     iApply (big_sepS_impl with "Hf2"). iIntros "!#" (x Hin) "(%f&%&?)". *)
+  (*     iExists _; iFrame. iPureIntro. rewrite map_filter_lookup_Some //. }     *)
+  (*   iSplitL "Hf1 HR1". *)
+  (*   { unfold has_fuels. *)
+  (*     rewrite dom_domain_restrict; *)
+  (*       [|set_solver -Hsamedoms Hsamedoms Hfueldom Hlocincl Hdomincl]. *)
+  (*     iFrame. *)
+  (*     iApply (big_sepS_impl with "Hf1"). iIntros "!#" (x Hin) "(%f&%&?)". *)
+  (*     iExists _; iFrame. iPureIntro. rewrite map_filter_lookup_Some //. } *)
+  (*   iSplitR; [iIntros; by iFrame | ]. *)
 
-    (* assert (maps_inverse_match _ (<[τ_new:=R2]> (<[ζ:=R1]> (ls_tmap δ1))) *)
+  (*   (* assert (maps_inverse_match _ (<[τ_new:=R2]> (<[ζ:=R1]> (ls_tmap δ1))) *) *)
     
-    assert (maps_inverse_match
-    (map_imap
-       (λ (ρ : fmrole M) (o : locale Λ),
-          if decide (ρ ∈ R2) then Some τ_new else Some o)
-       (ls_mapping δ1)) (<[τ_new:=R2]> (<[ζ:=R1]> (ls_tmap δ1)))) as MATCH.
-    { 
-      pose proof (ls_mapping_tmap_corr δ1 (LM := LM)) as Hminv. 
+  (*   assert (maps_inverse_match *)
+  (*   (map_imap *)
+  (*      (λ (ρ : fmrole M) (o : locale Λ), *)
+  (*         if decide (ρ ∈ R2) then Some τ_new else Some o) *)
+  (*      (ls_mapping δ1)) (<[τ_new:=R2]> (<[ζ:=R1]> (ls_tmap δ1)))) as MATCH. *)
+  (*   {  *)
+  (*     pose proof (ls_mapping_tmap_corr δ1 (LM := LM)) as Hminv.  *)
 
-        intros ρ ζ'. rewrite map_lookup_imap.
-        destruct (decide (ρ ∈ dom (ls_mapping δ1))) as [Hin|Hin].
-        + apply elem_of_dom in Hin as [ζ'' Hρ]. rewrite Hρ. simpl.
-          destruct (decide (ρ ∈ R2)) as [Hin'|Hin'].
-          * split.
-            -- intros. simplify_eq. rewrite lookup_insert. eauto.
-            -- intros (ks & Hlk & H'). destruct (decide (ζ' = τ_new)); first congruence.
-               rewrite lookup_insert_ne // in Hlk. exfalso.
-               assert (ρ ∈ dom fs).
-               { set_unfold. naive_solver. }
-               destruct (decide (ζ = ζ')); simplify_eq.
-               ** rewrite lookup_insert in Hlk. set_unfold. naive_solver.
-               ** rewrite lookup_insert_ne // in Hlk.
-                  assert (ζ = ζ'); last done.
-                  { eapply (maps_inverse_bij _ _ _ _ ks); eauto. }
-          * split.
-            -- intros ?. simplify_eq.
-               specialize (Hminv ρ ζ').
-               apply Hminv in Hρ as (?&?&?).
-               destruct (decide (ζ' = τ_new)).
-               { simplify_eq. apply not_elem_of_dom in Hnewζ.
-                 simpl in Hnewζ. rewrite -> Hnewζ in *. congruence. }
-               destruct (decide (ζ' = ζ)).
-               { simplify_eq. assert (ρ ∈ R1); first set_solver.
-                 exists R1. rewrite lookup_insert_ne // lookup_insert //. }
-               rewrite lookup_insert_ne // lookup_insert_ne //. eauto.
-            -- intros (ks&Hin&?).
-               destruct (decide (ζ' = τ_new)).
-               { simplify_eq. rewrite lookup_insert in Hin. set_solver. }
-               rewrite lookup_insert_ne // in Hin.
-               destruct (decide (ζ' = ζ)).
-               { simplify_eq. rewrite lookup_insert // in Hin.
-                 f_equal. simplify_eq.
-                 assert (ls_mapping δ1 !! ρ = Some ζ).
-                 { eapply Hminv. eexists _. split; eauto. set_unfold; naive_solver. }
-                 congruence. }
-               rewrite lookup_insert_ne // in Hin.
-               assert (ls_mapping δ1 !! ρ = Some ζ').
-               { eapply Hminv. eexists _. split; eauto. }
-               congruence.
-        + apply not_elem_of_dom in Hin. rewrite Hin /=. split; first done.
-          intros (?&Hin'&?). rewrite -ls_same_doms in Hdomincl.
-          apply not_elem_of_dom in Hin.
-          destruct (decide (ζ' = τ_new)).
-          { simplify_eq. rewrite lookup_insert in Hin'. simplify_eq.
-            set_unfold; naive_solver. }
-          rewrite lookup_insert_ne // in Hin'.
-          destruct (decide (ζ' = ζ)).
-          { simplify_eq. rewrite lookup_insert // in Hin'. simplify_eq.
-            set_unfold; naive_solver. }
-          rewrite lookup_insert_ne // in Hin'.
-          assert (ls_mapping δ1 !! ρ = Some ζ').
-          { eapply Hminv. eauto. }
-          apply not_elem_of_dom in Hin. congruence. }
+  (*       intros ρ ζ'. rewrite map_lookup_imap. *)
+  (*       destruct (decide (ρ ∈ dom (ls_mapping δ1))) as [Hin|Hin]. *)
+  (*       + apply elem_of_dom in Hin as [ζ'' Hρ]. rewrite Hρ. simpl. *)
+  (*         destruct (decide (ρ ∈ R2)) as [Hin'|Hin']. *)
+  (*         * split. *)
+  (*           -- intros. simplify_eq. rewrite lookup_insert. eauto. *)
+  (*           -- intros (ks & Hlk & H'). destruct (decide (ζ' = τ_new)); first congruence. *)
+  (*              rewrite lookup_insert_ne // in Hlk. exfalso. *)
+  (*              assert (ρ ∈ dom fs). *)
+  (*              { set_unfold. naive_solver. } *)
+  (*              destruct (decide (ζ = ζ')); simplify_eq. *)
+  (*              ** rewrite lookup_insert in Hlk. set_unfold. naive_solver. *)
+  (*              ** rewrite lookup_insert_ne // in Hlk. *)
+  (*                 assert (ζ = ζ'); last done. *)
+  (*                 { eapply (maps_inverse_bij _ _ _ _ ks); eauto. } *)
+  (*         * split. *)
+  (*           -- intros ?. simplify_eq. *)
+  (*              specialize (Hminv ρ ζ'). *)
+  (*              apply Hminv in Hρ as (?&?&?). *)
+  (*              destruct (decide (ζ' = τ_new)). *)
+  (*              { simplify_eq. apply not_elem_of_dom in Hnewζ. *)
+  (*                simpl in Hnewζ. rewrite -> Hnewζ in *. congruence. } *)
+  (*              destruct (decide (ζ' = ζ)). *)
+  (*              { simplify_eq. assert (ρ ∈ R1); first set_solver. *)
+  (*                exists R1. rewrite lookup_insert_ne // lookup_insert //. } *)
+  (*              rewrite lookup_insert_ne // lookup_insert_ne //. eauto. *)
+  (*           -- intros (ks&Hin&?). *)
+  (*              destruct (decide (ζ' = τ_new)). *)
+  (*              { simplify_eq. rewrite lookup_insert in Hin. set_solver. } *)
+  (*              rewrite lookup_insert_ne // in Hin. *)
+  (*              destruct (decide (ζ' = ζ)). *)
+  (*              { simplify_eq. rewrite lookup_insert // in Hin. *)
+  (*                f_equal. simplify_eq. *)
+  (*                assert (ls_mapping δ1 !! ρ = Some ζ). *)
+  (*                { eapply Hminv. eexists _. split; eauto. set_unfold; naive_solver. } *)
+  (*                congruence. } *)
+  (*              rewrite lookup_insert_ne // in Hin. *)
+  (*              assert (ls_mapping δ1 !! ρ = Some ζ'). *)
+  (*              { eapply Hminv. eexists _. split; eauto. } *)
+  (*              congruence. *)
+  (*       + apply not_elem_of_dom in Hin. rewrite Hin /=. split; first done. *)
+  (*         intros (?&Hin'&?). rewrite -ls_same_doms in Hdomincl. *)
+  (*         apply not_elem_of_dom in Hin. *)
+  (*         destruct (decide (ζ' = τ_new)). *)
+  (*         { simplify_eq. rewrite lookup_insert in Hin'. simplify_eq. *)
+  (*           set_unfold; naive_solver. } *)
+  (*         rewrite lookup_insert_ne // in Hin'. *)
+  (*         destruct (decide (ζ' = ζ)). *)
+  (*         { simplify_eq. rewrite lookup_insert // in Hin'. simplify_eq. *)
+  (*           set_unfold; naive_solver. } *)
+  (*         rewrite lookup_insert_ne // in Hin'. *)
+  (*         assert (ls_mapping δ1 !! ρ = Some ζ'). *)
+  (*         { eapply Hminv. eauto. } *)
+  (*         apply not_elem_of_dom in Hin. congruence. } *)
 
-    iSplitL "Ham Haf Hamod HFR".
-    { iExists FR; simpl.
-      rewrite build_LS_ext_spec_st build_LS_ext_spec_tmap build_LS_ext_spec_fuel.
-      iFrame "Ham Hamod HFR".
-      iSplit.
-      - iApply (auth_fuel_is_proper with "Haf"). unfold fuel_apply.
-        rewrite -leibniz_equiv_iff. intros ρ. rewrite !map_lookup_imap.
-        rewrite Hunioneq dom_fmap_L difference_diag_L difference_empty_L.
-        rewrite lookup_gset_to_gmap.
-        destruct (decide (ρ ∈ dom (ls_fuel δ1) ∪ dom fs)) as [Hin|Hin].
-        + rewrite option_guard_True //=.
-          assert (Hmap: ρ ∈ dom (ls_fuel δ1)).
-          { set_unfold. naive_solver. }
-          destruct (decide (ρ ∈ dom fs)) as [Hinfs|Hinfs].
-          * apply elem_of_dom in Hmap as [? Hinfuels]. rewrite Hinfuels /=.
-            rewrite Hfuels in Hinfuels; last set_solver.
-            rewrite lookup_fmap in Hinfuels.
-            rewrite leibniz_equiv_iff.
-            rewrite -lookup_fmap in Hinfuels.
-            rewrite lookup_fmap_Some in Hinfuels.
-            destruct Hinfuels as [y [<- Hinfuels]].
-            rewrite Hinfuels. f_equiv. lia.
-          * apply elem_of_dom in Hmap as [? Hinfuels].
-            rewrite Hinfuels //.
-        + rewrite option_guard_False //=.
-          rewrite -> not_elem_of_union in Hin. destruct Hin as [Hin ?].
-          rewrite -> not_elem_of_dom in Hin. rewrite Hin //.
-      - iPureIntro. split. 
-        { intros. eapply tids_dom_fork_step; eauto.
-          2: admit. 
-          congruence. }
-        { rewrite map_imap_dom_eq // => ρ f Hin. by destruct (decide (ρ ∈ R1 ∪ R2)). }
-    }
-    iSplit; first done.
-    iSplit; last first.
-    { iPureIntro.
-      eapply tids_smaller_fork_step; eauto.
-      2: admit. 
-      erewrite build_LS_ext_spec_mapping; eauto. }
-    iSplit.
-    { iPureIntro. destruct (map_choose _ Hnemp) as [ρ[??]]. exists ρ.
-      eapply ls_mapping_tmap_corr. 
-      (* apply Hminv. *)
-      eexists _. split; eauto. apply elem_of_dom. eauto. }
-    iSplit.
-    { iPureIntro. intros ρ Hlive Hlive' Hmd. simpl. inversion Hmd; simplify_eq.
-      - rewrite build_LS_ext_spec_fuel. 
-        rewrite map_lookup_imap.
-        assert (Hin: ρ ∈ dom (ls_fuel δ1)).
-        { rewrite -ls_same_doms elem_of_dom. eauto. }
-        apply elem_of_dom in Hin. destruct Hin as [f' Hin'].
-        rewrite Hin' /=.
-        destruct (decide (ρ ∈ R1 ∪ R2)) as [Hin''|Hin''].
-        { rewrite dom_fmap_L -Hunioneq in Hfuels.
-          specialize (Hfuels _ Hin''). rewrite lookup_fmap Hin' in Hfuels.
-          destruct (fs !! ρ); simplify_eq. simpl in Hfuels. injection Hfuels.
-          intros ->. simpl. lia. }
-        symmetry in Hsametid. eapply ls_mapping_tmap_corr in Hsametid as (?&?&?).
-        set_unfold; naive_solver.
-      - rewrite build_LS_ext_spec_fuel. 
-        rewrite map_lookup_imap. simpl in *. clear Hmd.
-        erewrite build_LS_ext_spec_mapping in Hissome, Hneqtid.
-        2, 3: by eauto. 
-        destruct (decide (ρ ∈ dom (ls_mapping δ1))) as [Hin|Hin]; last first.
-        { apply not_elem_of_dom in Hin.
-          rewrite map_lookup_imap Hin //= in Hissome. by inversion Hissome. }
-        apply elem_of_dom in Hin as [ζ' Hin'].
-        rewrite map_lookup_imap Hin' /= in Hneqtid.
-        destruct (decide (ρ ∈ R2)) as [Hin''|Hin'']; last done.
-        rewrite Hfuels; last (set_unfold; naive_solver). rewrite lookup_fmap.
-        assert (Hindom: ρ ∈ dom fs); first by set_unfold; naive_solver.
-        apply elem_of_dom in Hindom as [f Hindom]. rewrite Hindom /= decide_True /=; [lia|set_unfold; naive_solver]. }
-    iSplit.
-    { iPureIntro. intros ρ' Hρ' _. simpl. left.
-      rewrite build_LS_ext_spec_fuel. 
-      rewrite map_lookup_imap. rewrite elem_of_dom in Hρ'.
-      destruct Hρ' as [f Hf]. rewrite Hf /=. destruct (decide ((ρ' ∈ R1 ∪ R2))); simpl; lia. }
-    rewrite build_LS_ext_spec_fuel build_LS_ext_spec_st. 
-    iSplit; [simpl| done]. rewrite map_imap_dom_eq //.
-    by intros ρ??; destruct (decide (ρ ∈ R1 ∪ R2)).
-  Admitted. 
+  (*   iSplitL "Ham Haf Hamod HFR". *)
+  (*   { iExists FR; simpl. *)
+  (*     rewrite build_LS_ext_spec_st build_LS_ext_spec_tmap build_LS_ext_spec_fuel. *)
+  (*     iFrame "Ham Hamod HFR". *)
+  (*     iSplit. *)
+  (*     - iApply (auth_fuel_is_proper with "Haf"). unfold fuel_apply. *)
+  (*       rewrite -leibniz_equiv_iff. intros ρ. rewrite !map_lookup_imap. *)
+  (*       rewrite Hunioneq dom_fmap_L difference_diag_L difference_empty_L. *)
+  (*       rewrite lookup_gset_to_gmap. *)
+  (*       destruct (decide (ρ ∈ dom (ls_fuel δ1) ∪ dom fs)) as [Hin|Hin]. *)
+  (*       + rewrite option_guard_True //=. *)
+  (*         assert (Hmap: ρ ∈ dom (ls_fuel δ1)). *)
+  (*         { set_unfold. naive_solver. } *)
+  (*         destruct (decide (ρ ∈ dom fs)) as [Hinfs|Hinfs]. *)
+  (*         * apply elem_of_dom in Hmap as [? Hinfuels]. rewrite Hinfuels /=. *)
+  (*           rewrite Hfuels in Hinfuels; last set_solver. *)
+  (*           rewrite lookup_fmap in Hinfuels. *)
+  (*           rewrite leibniz_equiv_iff. *)
+  (*           rewrite -lookup_fmap in Hinfuels. *)
+  (*           rewrite lookup_fmap_Some in Hinfuels. *)
+  (*           destruct Hinfuels as [y [<- Hinfuels]]. *)
+  (*           rewrite Hinfuels. f_equiv. lia. *)
+  (*         * apply elem_of_dom in Hmap as [? Hinfuels]. *)
+  (*           rewrite Hinfuels //. *)
+  (*       + rewrite option_guard_False //=. *)
+  (*         rewrite -> not_elem_of_union in Hin. destruct Hin as [Hin ?]. *)
+  (*         rewrite -> not_elem_of_dom in Hin. rewrite Hin //. *)
+  (*     - iPureIntro. split.  *)
+  (*       { intros. eapply tids_dom_fork_step; eauto. *)
+  (*         2: admit.  *)
+  (*         congruence. } *)
+  (*       { rewrite map_imap_dom_eq // => ρ f Hin. by destruct (decide (ρ ∈ R1 ∪ R2)). } *)
+  (*   } *)
+  (*   iSplit; first done. *)
+  (*   iSplit; last first. *)
+  (*   { iPureIntro. *)
+  (*     eapply tids_smaller_fork_step; eauto. *)
+  (*     2: admit.  *)
+  (*     erewrite build_LS_ext_spec_mapping; eauto. } *)
+  (*   iSplit. *)
+  (*   { iPureIntro. destruct (map_choose _ Hnemp) as [ρ[??]]. exists ρ. *)
+  (*     eapply ls_mapping_tmap_corr.  *)
+  (*     (* apply Hminv. *) *)
+  (*     eexists _. split; eauto. apply elem_of_dom. eauto. } *)
+  (*   iSplit. *)
+  (*   { iPureIntro. intros ρ Hlive Hlive' Hmd. simpl. inversion Hmd; simplify_eq. *)
+  (*     - rewrite build_LS_ext_spec_fuel.  *)
+  (*       rewrite map_lookup_imap. *)
+  (*       assert (Hin: ρ ∈ dom (ls_fuel δ1)). *)
+  (*       { rewrite -ls_same_doms elem_of_dom. eauto. } *)
+  (*       apply elem_of_dom in Hin. destruct Hin as [f' Hin']. *)
+  (*       rewrite Hin' /=. *)
+  (*       destruct (decide (ρ ∈ R1 ∪ R2)) as [Hin''|Hin'']. *)
+  (*       { rewrite dom_fmap_L -Hunioneq in Hfuels. *)
+  (*         specialize (Hfuels _ Hin''). rewrite lookup_fmap Hin' in Hfuels. *)
+  (*         destruct (fs !! ρ); simplify_eq. simpl in Hfuels. injection Hfuels. *)
+  (*         intros ->. simpl. lia. } *)
+  (*       symmetry in Hsametid. eapply ls_mapping_tmap_corr in Hsametid as (?&?&?). *)
+  (*       set_unfold; naive_solver. *)
+  (*     - rewrite build_LS_ext_spec_fuel.  *)
+  (*       rewrite map_lookup_imap. simpl in *. clear Hmd. *)
+  (*       erewrite build_LS_ext_spec_mapping in Hissome, Hneqtid. *)
+  (*       2, 3: by eauto.  *)
+  (*       destruct (decide (ρ ∈ dom (ls_mapping δ1))) as [Hin|Hin]; last first. *)
+  (*       { apply not_elem_of_dom in Hin. *)
+  (*         rewrite map_lookup_imap Hin //= in Hissome. by inversion Hissome. } *)
+  (*       apply elem_of_dom in Hin as [ζ' Hin']. *)
+  (*       rewrite map_lookup_imap Hin' /= in Hneqtid. *)
+  (*       destruct (decide (ρ ∈ R2)) as [Hin''|Hin'']; last done. *)
+  (*       rewrite Hfuels; last (set_unfold; naive_solver). rewrite lookup_fmap. *)
+  (*       assert (Hindom: ρ ∈ dom fs); first by set_unfold; naive_solver. *)
+  (*       apply elem_of_dom in Hindom as [f Hindom]. rewrite Hindom /= decide_True /=; [lia|set_unfold; naive_solver]. } *)
+  (*   iSplit. *)
+  (*   { iPureIntro. intros ρ' Hρ' _. simpl. left. *)
+  (*     rewrite build_LS_ext_spec_fuel.  *)
+  (*     rewrite map_lookup_imap. rewrite elem_of_dom in Hρ'. *)
+  (*     destruct Hρ' as [f Hf]. rewrite Hf /=. destruct (decide ((ρ' ∈ R1 ∪ R2))); simpl; lia. } *)
+  (*   rewrite build_LS_ext_spec_fuel build_LS_ext_spec_st.  *)
+  (*   iSplit; [simpl| done]. rewrite map_imap_dom_eq //. *)
+  (*   by intros ρ??; destruct (decide (ρ ∈ R1 ∪ R2)). *)
+  (* Admitted.  *)
 
-  Ltac by_contradiction :=
-    match goal with
-    | |- ?goal => destruct_decide (decide (goal)); first done; exfalso
-    end.
+  (* Ltac by_contradiction := *)
+  (*   match goal with *)
+  (*   | |- ?goal => destruct_decide (decide (goal)); first done; exfalso *)
+  (*   end. *)
 
-  (* TODO: move to upstream *)
-  Lemma disjoint_subseteq:
-  ∀ {A C : Type} {H : ElemOf A C} {H0 : Empty C} {H1 : Singleton A C} 
-    {H2 : Union C} {H3 : Intersection C} {H4 : Difference C},
-    `{Set_ A C} → ∀ X1 X2 Y1 Y2: C, X1 ⊆ Y1 -> X2 ⊆ Y2 → Y1 ## Y2 -> X1 ## X2.
-  Proof. intros. set_solver. Qed. 
+  (* (* TODO: move to upstream *) *)
+  (* Lemma disjoint_subseteq: *)
+  (* ∀ {A C : Type} {H : ElemOf A C} {H0 : Empty C} {H1 : Singleton A C}  *)
+  (*   {H2 : Union C} {H3 : Intersection C} {H4 : Difference C}, *)
+  (*   `{Set_ A C} → ∀ X1 X2 Y1 Y2: C, X1 ⊆ Y1 -> X2 ⊆ Y2 → Y1 ## Y2 -> X1 ## X2. *)
+  (* Proof. intros. set_solver. Qed.  *)
 
-  Lemma union_intersection_difference_equiv_L:
-  ∀ {A C : Type} {H : ElemOf A C} {H0 : Empty C} {H1 : Singleton A C} 
-    {H2 : Union C} {H3 : Intersection C} {H4 : Difference C},
-    Set_ A C → LeibnizEquiv C →
-    ∀ X Y: C, (forall y, Decision (y ∈ Y)) ->
-    X ≡ X ∩ Y ∪ X ∖ Y.
-  Proof.
-    intros. apply set_equiv_subseteq. split; [| set_solver].
-    apply elem_of_subseteq. intros x ?.
-    destruct (decide (x ∈ Y)); set_solver.
-  Qed. 
+  (* Lemma union_intersection_difference_equiv_L: *)
+  (* ∀ {A C : Type} {H : ElemOf A C} {H0 : Empty C} {H1 : Singleton A C}  *)
+  (*   {H2 : Union C} {H3 : Intersection C} {H4 : Difference C}, *)
+  (*   Set_ A C → LeibnizEquiv C → *)
+  (*   ∀ X Y: C, (forall y, Decision (y ∈ Y)) -> *)
+  (*   X ≡ X ∩ Y ∪ X ∖ Y. *)
+  (* Proof. *)
+  (*   intros. apply set_equiv_subseteq. split; [| set_solver]. *)
+  (*   apply elem_of_subseteq. intros x ?. *)
+  (*   destruct (decide (x ∈ Y)); set_solver. *)
+  (* Qed.  *)
 
-  Lemma tids_smaller_model_step c1 c2 ζ δ1 δ2
-    (Hstep: locale_step c1 (Some ζ) c2)
-    (Hless: tids_smaller c1.1 δ1)
-    (* S is a subset of dom (ls_fuel δ1);
-       missing roles are those that are dropped by ζ;
-       new roles get assigned here *)
-    (MAP2: exists f (S: gset (fmrole M)),
-        ls_mapping δ2 = map_imap
-          (λ (ρ' : fmrole M) (_ : nat),
-             if decide (ρ' ∈ dom (ls_fuel δ1))
-             then ls_mapping δ1 !! ρ'
-             else Some ζ)
-          (gset_to_gmap f S)
-    )
-    :
-    tids_smaller c2.1 δ2 (M := M).
-  Proof. 
-    unfold tids_smaller; simpl.
-    destruct MAP2 as (?&S&->). 
-    intros ρ' ? Hmim.
-    rewrite map_lookup_imap in Hmim. rewrite lookup_gset_to_gmap in Hmim.
-    destruct (decide (ρ' ∈ S)); last by rewrite option_guard_False in Hmim.
-    rewrite option_guard_True //= in Hmim.
-    destruct (decide (ρ' ∈ dom (ls_fuel δ1))).
-    + inversion Hstep; simplify_eq.
-      eapply from_locale_step =>//. by eapply Hless.
-    + simplify_eq.
-      inversion Hstep; simplify_eq.
-      eapply from_locale_step =>//. unfold from_locale. rewrite from_locale_from_Some //.
-      apply prefixes_from_spec. exists t1, t2. by list_simplifier.
-  Qed. 
+  (* Lemma tids_smaller_model_step c1 c2 ζ δ1 δ2 *)
+  (*   (Hstep: locale_step c1 (Some ζ) c2) *)
+  (*   (Hless: tids_smaller c1.1 δ1) *)
+  (*   (* S is a subset of dom (ls_fuel δ1); *)
+  (*      missing roles are those that are dropped by ζ; *)
+  (*      new roles get assigned here *) *)
+  (*   (MAP2: exists f (S: gset (fmrole M)), *)
+  (*       ls_mapping δ2 = map_imap *)
+  (*         (λ (ρ' : fmrole M) (_ : nat), *)
+  (*            if decide (ρ' ∈ dom (ls_fuel δ1)) *)
+  (*            then ls_mapping δ1 !! ρ' *)
+  (*            else Some ζ) *)
+  (*         (gset_to_gmap f S) *)
+  (*   ) *)
+  (*   : *)
+  (*   tids_smaller c2.1 δ2 (M := M). *)
+  (* Proof.  *)
+  (*   unfold tids_smaller; simpl. *)
+  (*   destruct MAP2 as (?&S&->).  *)
+  (*   intros ρ' ? Hmim. *)
+  (*   rewrite map_lookup_imap in Hmim. rewrite lookup_gset_to_gmap in Hmim. *)
+  (*   destruct (decide (ρ' ∈ S)); last by rewrite option_guard_False in Hmim. *)
+  (*   rewrite option_guard_True //= in Hmim. *)
+  (*   destruct (decide (ρ' ∈ dom (ls_fuel δ1))). *)
+  (*   + inversion Hstep; simplify_eq. *)
+  (*     eapply from_locale_step =>//. by eapply Hless. *)
+  (*   + simplify_eq. *)
+  (*     inversion Hstep; simplify_eq. *)
+  (*     eapply from_locale_step =>//. unfold from_locale. rewrite from_locale_from_Some //. *)
+  (*     apply prefixes_from_spec. exists t1, t2. by list_simplifier. *)
+  (* Qed.  *)
 
-  Lemma tids_restrict_model_step c1 c2 ζ
-    (tmap1 tmap2: gmap (locale Λ) (gset (fmrole M))) ρ
-    (D2: gset (fmrole M))
-    (Hstep: locale_step c1 (Some ζ) c2)
-    (* Hfuelsval : valid_new_fuelmap fs1 fs2 s1 s2 ρ *)
-  (* Hxdom : ∀ ρ : fmrole M, ls_mapping δ1 !! ρ = Some ζ ↔ ρ ∈ dom fs1 *)
-    (* TODO: D2 = dom fs2 *)
-    (Hsmall: ∀ ζ : locale Λ,
-        ζ ∉ locales_of_list c1.1 → tmap1 !! ζ = None)
-    (* (Hfs1: ls_mapping δ1 !! ρ = Some ζ) *)
-    (Hfs1: exists R, tmap1 !! ζ = Some R /\ ρ ∈ R)
-    (TMAP2: tmap2 = <[ζ:= D2]> (tmap1)):
-  ∀ ζ0 : locale Λ,
-    ζ0 ∉ locales_of_list c2.1 → tmap2 !! ζ0 = None.
-  Proof.
-    intros ζ' ?.
-    destruct c1, c2. simpl in *. 
-    pose proof (locales_of_list_step_incl _ _ _ _ _ Hstep). simpl.
-    rewrite TMAP2. 
-    rewrite lookup_insert_ne; first by apply Hsmall; set_solver.
-    intros <-.
-    (* TODO: use this to prove Hfs1 premise *)
-    (* destruct Hfuelsval as (_&_&Hfs1&_). *)
-    (* rewrite <-Hxdom in Hfs1. *)
+  (* Lemma tids_restrict_model_step c1 c2 ζ *)
+  (*   (tmap1 tmap2: gmap (locale Λ) (gset (fmrole M))) ρ *)
+  (*   (D2: gset (fmrole M)) *)
+  (*   (Hstep: locale_step c1 (Some ζ) c2) *)
+  (*   (* Hfuelsval : valid_new_fuelmap fs1 fs2 s1 s2 ρ *) *)
+  (* (* Hxdom : ∀ ρ : fmrole M, ls_mapping δ1 !! ρ = Some ζ ↔ ρ ∈ dom fs1 *) *)
+  (*   (* TODO: D2 = dom fs2 *) *)
+  (*   (Hsmall: ∀ ζ : locale Λ, *)
+  (*       ζ ∉ locales_of_list c1.1 → tmap1 !! ζ = None) *)
+  (*   (* (Hfs1: ls_mapping δ1 !! ρ = Some ζ) *) *)
+  (*   (Hfs1: exists R, tmap1 !! ζ = Some R /\ ρ ∈ R) *)
+  (*   (TMAP2: tmap2 = <[ζ:= D2]> (tmap1)): *)
+  (* ∀ ζ0 : locale Λ, *)
+  (*   ζ0 ∉ locales_of_list c2.1 → tmap2 !! ζ0 = None. *)
+  (* Proof. *)
+  (*   intros ζ' ?. *)
+  (*   destruct c1, c2. simpl in *.  *)
+  (*   pose proof (locales_of_list_step_incl _ _ _ _ _ Hstep). simpl. *)
+  (*   rewrite TMAP2.  *)
+  (*   rewrite lookup_insert_ne; first by apply Hsmall; set_solver. *)
+  (*   intros <-. *)
+  (*   (* TODO: use this to prove Hfs1 premise *) *)
+  (*   (* destruct Hfuelsval as (_&_&Hfs1&_). *) *)
+  (*   (* rewrite <-Hxdom in Hfs1. *) *)
 
-    (* apply (ls_mapping_tmap_corr (LM := LM)) in Hfs1 as (?&HM&?). *)
-    rewrite Hsmall // in Hfs1; set_solver.
-  Qed. 
+  (*   (* apply (ls_mapping_tmap_corr (LM := LM)) in Hfs1 as (?&HM&?). *) *)
+  (*   rewrite Hsmall // in Hfs1; set_solver. *)
+  (* Qed.  *)
     
 
-  Lemma actual_update_step_still_alive
-        tp1 tp2 σ1 σ2 s1 s2 fs1 fs2 ρ (δ1 : LM) ζ fr1 fr_stash:
-    (live_roles _ s2 ∖ live_roles _ s1) ⊆ fr1 ->
-    fr_stash ⊆ dom fs1 ->
-    (live_roles _ s1) ∩ (fr_stash ∖ {[ ρ ]}) = ∅ ->
-    dom fs2 ∩ fr_stash = ∅ ->
-    (* trace_last extr = (tp1, σ1) → *)
-    (* trace_last auxtr = δ1 -> *)
-    locale_step (tp1, σ1) (Some ζ) (tp2, σ2) ->
-    fmtrans _ s1 (Some ρ) s2 -> valid_new_fuelmap fs1 fs2 s1 s2 ρ (LM := LM) ->
-    has_fuels ζ fs1 -∗ frag_model_is s1 -∗ model_state_interp (tp1, σ1) δ1 -∗
-    frag_free_roles_are fr1
-    ==∗ ∃ (δ2: LM) ℓ,
-        ⌜labels_match (Some ζ) ℓ ∧
-          (* valid_state_evolution_fairness (extr :tr[Some ζ]: (tp2, σ2)) (auxtr :tr[ℓ]: δ2) *)
-          valid_evolution_step (Some ζ) (tp2, σ2) δ1 ℓ δ2 (LM := LM)
-            ⌝
-        ∗ has_fuels ζ fs2 ∗ frag_model_is s2 ∗ model_state_interp (tp2, σ2) δ2 ∗
-        frag_free_roles_are (fr1 ∖ (live_roles _ s2 ∖ live_roles _ s1) ∪ fr_stash).
-  Proof.
-    iIntros (Hfr_new Hstash_own Hstash_dis Hstash_rem Hstep Htrans Hfuelsval) "Hfuel Hmod Hsi Hfr1".
+  (* Lemma actual_update_step_still_alive *)
+  (*       tp1 tp2 σ1 σ2 s1 s2 fs1 fs2 ρ (δ1 : LM) ζ fr1 fr_stash: *)
+  (*   (live_roles _ s2 ∖ live_roles _ s1) ⊆ fr1 -> *)
+  (*   fr_stash ⊆ dom fs1 -> *)
+  (*   (live_roles _ s1) ∩ (fr_stash ∖ {[ ρ ]}) = ∅ -> *)
+  (*   dom fs2 ∩ fr_stash = ∅ -> *)
+  (*   (* trace_last extr = (tp1, σ1) → *) *)
+  (*   (* trace_last auxtr = δ1 -> *) *)
+  (*   locale_step (tp1, σ1) (Some ζ) (tp2, σ2) -> *)
+  (*   fmtrans _ s1 (Some ρ) s2 -> valid_new_fuelmap fs1 fs2 s1 s2 ρ (LM := LM) -> *)
+  (*   has_fuels ζ fs1 -∗ frag_model_is s1 -∗ model_state_interp (tp1, σ1) δ1 -∗ *)
+  (*   frag_free_roles_are fr1 *)
+  (*   ==∗ ∃ (δ2: LM) ℓ, *)
+  (*       ⌜labels_match (Some ζ) ℓ ∧ *)
+  (*         (* valid_state_evolution_fairness (extr :tr[Some ζ]: (tp2, σ2)) (auxtr :tr[ℓ]: δ2) *) *)
+  (*         valid_evolution_step (Some ζ) (tp2, σ2) δ1 ℓ δ2 (LM := LM) *)
+  (*           ⌝ *)
+  (*       ∗ has_fuels ζ fs2 ∗ frag_model_is s2 ∗ model_state_interp (tp2, σ2) δ2 ∗ *)
+  (*       frag_free_roles_are (fr1 ∖ (live_roles _ s2 ∖ live_roles _ s1) ∪ fr_stash). *)
+  (* Proof. *)
+  (*   iIntros (Hfr_new Hstash_own Hstash_dis Hstash_rem Hstep Htrans Hfuelsval) "Hfuel Hmod Hsi Hfr1". *)
 
-    assert (Hfsne: fs1 ≠ ∅).
-    { destruct Hfuelsval as (_&_&?&_). intros ->. set_solver. }
+  (*   assert (Hfsne: fs1 ≠ ∅). *)
+  (*   { destruct Hfuelsval as (_&_&?&_). intros ->. set_solver. } *)
 
-    iDestruct (has_fuel_in with "Hfuel Hsi") as "%Hxdom"; eauto.
-    iDestruct (has_fuel_fuel with "Hfuel Hsi") as %Hfuel; eauto.
-    iDestruct (model_state_interp_tids_smaller with "Hsi") as %Hless.
+  (*   iDestruct (has_fuel_in with "Hfuel Hsi") as "%Hxdom"; eauto. *)
+  (*   iDestruct (has_fuel_fuel with "Hfuel Hsi") as %Hfuel; eauto. *)
+  (*   iDestruct (model_state_interp_tids_smaller with "Hsi") as %Hless. *)
 
-    iDestruct "Hsi" as "(%FR&Hafuel&Hamapping&HFR&%Hsmall&Hamod&%HFR)".
-    iDestruct (model_agree with "Hamod Hmod") as "%Heq".
+  (*   iDestruct "Hsi" as "(%FR&Hafuel&Hamapping&HFR&%Hsmall&Hamod&%HFR)". *)
+  (*   iDestruct (model_agree with "Hamod Hmod") as "%Heq". *)
 
-    iDestruct (free_roles_inclusion with "HFR Hfr1") as %HfrFR.
+  (*   iDestruct (free_roles_inclusion with "HFR Hfr1") as %HfrFR. *)
 
-    set (new_mapping := map_imap
-                    (λ ρ' _, if decide (ρ' ∈ dom $ ls_fuel δ1) then ls_mapping δ1 !! ρ' else Some ζ)
-                    (gset_to_gmap 333 ((dom (ls_fuel δ1) ∪ dom fs2) ∖ (dom fs1 ∖ dom fs2)))). 
-    assert (Hsamedoms: dom new_mapping
-              =
-               dom (update_fuel_resource δ1 fs1 fs2 s2)).
-    { unfold update_fuel_resource, fuel_apply. rewrite -leibniz_equiv_iff.
-      intros ρ'; split.
-      - intros Hin. destruct (decide (ρ' ∈ dom fs2)) as [[f Hin1]%elem_of_dom|Hin1].
-        + apply elem_of_dom. eexists f. rewrite map_lookup_imap lookup_gset_to_gmap option_guard_True //=.
-          rewrite decide_True //. apply elem_of_dom. rewrite Hin1; eauto.
-          rewrite map_imap_dom_eq dom_gset_to_gmap in Hin; first set_solver.
-          intros ρ0??. destruct (decide (ρ0 ∈ dom $ ls_fuel δ1)); [|done].
-          apply elem_of_dom. rewrite ls_same_doms. SS.
-        + rewrite map_imap_dom_eq dom_gset_to_gmap; last first.
-          { intros ρ0 ? Hin0. destruct (decide (ρ0 ∈ dom fs2)) as [|Hnotin]; apply elem_of_dom; first done.
-            unfold valid_new_fuelmap in Hfuelsval.
-            destruct Hfuelsval as (_&_&_&_& Hdomfs2). set_solver. }
+  (*   set (new_mapping := map_imap *)
+  (*                   (λ ρ' _, if decide (ρ' ∈ dom $ ls_fuel δ1) then ls_mapping δ1 !! ρ' else Some ζ) *)
+  (*                   (gset_to_gmap 333 ((dom (ls_fuel δ1) ∪ dom fs2) ∖ (dom fs1 ∖ dom fs2)))).  *)
+  (*   assert (Hsamedoms: dom new_mapping *)
+  (*             = *)
+  (*              dom (update_fuel_resource δ1 fs1 fs2 s2)). *)
+  (*   { unfold update_fuel_resource, fuel_apply. rewrite -leibniz_equiv_iff. *)
+  (*     intros ρ'; split. *)
+  (*     - intros Hin. destruct (decide (ρ' ∈ dom fs2)) as [[f Hin1]%elem_of_dom|Hin1]. *)
+  (*       + apply elem_of_dom. eexists f. rewrite map_lookup_imap lookup_gset_to_gmap option_guard_True //=. *)
+  (*         rewrite decide_True //. apply elem_of_dom. rewrite Hin1; eauto. *)
+  (*         rewrite map_imap_dom_eq dom_gset_to_gmap in Hin; first set_solver. *)
+  (*         intros ρ0??. destruct (decide (ρ0 ∈ dom $ ls_fuel δ1)); [|done]. *)
+  (*         apply elem_of_dom. rewrite ls_same_doms. SS. *)
+  (*       + rewrite map_imap_dom_eq dom_gset_to_gmap; last first. *)
+  (*         { intros ρ0 ? Hin0. destruct (decide (ρ0 ∈ dom fs2)) as [|Hnotin]; apply elem_of_dom; first done. *)
+  (*           unfold valid_new_fuelmap in Hfuelsval. *)
+  (*           destruct Hfuelsval as (_&_&_&_& Hdomfs2). set_solver. } *)
 
-          rewrite map_imap_dom_eq dom_gset_to_gmap in Hin; first set_solver.
-          intros ρ0??. destruct (decide (ρ0 ∈ dom $ ls_fuel δ1)); [|done].
-          apply elem_of_dom. rewrite ls_same_doms. SS.
-      - intros [f Hin]%elem_of_dom. rewrite map_lookup_imap in Hin.
-        rewrite map_imap_dom_eq dom_gset_to_gmap.
-        + by_contradiction. rewrite lookup_gset_to_gmap option_guard_False // in Hin.
-        + intros ρ0??. destruct (decide (ρ0 ∈ dom $ ls_fuel δ1)); [|done].
-          apply elem_of_dom. rewrite ls_same_doms. SS. }
+  (*         rewrite map_imap_dom_eq dom_gset_to_gmap in Hin; first set_solver. *)
+  (*         intros ρ0??. destruct (decide (ρ0 ∈ dom $ ls_fuel δ1)); [|done]. *)
+  (*         apply elem_of_dom. rewrite ls_same_doms. SS. *)
+  (*     - intros [f Hin]%elem_of_dom. rewrite map_lookup_imap in Hin. *)
+  (*       rewrite map_imap_dom_eq dom_gset_to_gmap. *)
+  (*       + by_contradiction. rewrite lookup_gset_to_gmap option_guard_False // in Hin. *)
+  (*       + intros ρ0??. destruct (decide (ρ0 ∈ dom $ ls_fuel δ1)); [|done]. *)
+  (*         apply elem_of_dom. rewrite ls_same_doms. SS. } *)
 
-    assert (Hnewdom: dom (update_fuel_resource δ1 fs1 fs2 s2) =
-                       (dom (ls_fuel δ1) ∪ dom fs2) ∖ (dom fs1 ∖ dom fs2)).
-    { unfold update_fuel_resource, fuel_apply. rewrite map_imap_dom_eq ?dom_gset_to_gmap //.
-      intros ρ' _ Hin. destruct (decide (ρ' ∈ dom fs2)); apply elem_of_dom =>//. set_solver. }
+  (*   assert (Hnewdom: dom (update_fuel_resource δ1 fs1 fs2 s2) = *)
+  (*                      (dom (ls_fuel δ1) ∪ dom fs2) ∖ (dom fs1 ∖ dom fs2)). *)
+  (*   { unfold update_fuel_resource, fuel_apply. rewrite map_imap_dom_eq ?dom_gset_to_gmap //. *)
+  (*     intros ρ' _ Hin. destruct (decide (ρ' ∈ dom fs2)); apply elem_of_dom =>//. set_solver. } *)
 
-    assert (Hfueldom: live_roles _ s2 ⊆ dom $ update_fuel_resource δ1 fs1 fs2 s2).
-    { rewrite -Hsamedoms map_imap_dom_eq dom_gset_to_gmap //.
-      { epose proof ls_fuel_dom as Hfueldom. intros ρ' Hin.
-        destruct Hfuelsval as (?&?&?&?&?&Hdom_le).
-        destruct (decide (ρ' ∈ live_roles _ δ1)).
-        - apply elem_of_difference.
-          split; [set_solver -Hnewdom Hsamedoms Hdom_le|].
-          intros [? Habs]%elem_of_difference.
-          destruct (decide (ρ' = ρ)).
-          + simplify_eq. apply not_elem_of_dom in Habs.
-            rewrite -> Habs in *. simpl in *. eauto.
-          + apply Habs.
-            assert (ρ' ∈ dom fs1 ∖ {[ρ]}); set_solver -Hnewdom Hsamedoms.
-        - apply elem_of_difference.
-          split; [apply elem_of_union; right; set_unfold; naive_solver|
-                   set_unfold; naive_solver]. }
-      intros ρ0??. destruct (decide (ρ0 ∈ dom $ ls_fuel δ1)); [|done].
-      apply elem_of_dom. rewrite ls_same_doms. SS. }
-    (* iExists {| *)
-    (*   ls_under := s2; *)
-    (*   ls_fuel :=  _; *)
-    (*   ls_fuel_dom := Hfueldom; *)
-    (*   ls_mapping := _; *)
-    (*   ls_same_doms := Hsamedoms; *)
-    (* |}.  *)
-    iExists (build_LS_ext s2 _ Hfueldom (<[ζ:=dom fs2]> (ls_tmap δ1 (LM := LM))) _ _ (LM := LM)).
-    iExists (Take_step ρ ζ).
-    (* Unshelve. *)
-    iMod (update_has_fuels _ fs1 fs2 with "Hfuel Hafuel Hamapping") as "(Hafuel & Hfuel & Hmapping)".
-    { set_solver. }
-    { unfold valid_new_fuelmap in Hfuelsval.
-      destruct Hfuelsval as (_&_&?&?& Hfs2_inf&Hfs2_sup).
-      apply elem_of_equiv_empty_L => ρ0 Hin.
-      apply elem_of_intersection in Hin as [Hin1 Hin2].
-      apply elem_of_difference in Hin1 as [Hin11 Hin12].
-      assert (ρ0 ∈ live_roles _ s2 ∖ live_roles _ s1)
-             by set_solver -Hsamedoms Hnewdom.
-      assert (ρ0 ∈ fr1) by set_solver -Hsamedoms Hnewdom.
-      assert (ρ0 ∈ FR) by set_solver -Hsamedoms Hnewdom.
-      assert (ρ0 ∉ dom (ls_fuel δ1)) by set_solver -Hsamedoms Hnewdom.
-      done. }
-    iMod (update_model s2 with "Hamod Hmod") as "[Hamod Hmod]".
+  (*   assert (Hfueldom: live_roles _ s2 ⊆ dom $ update_fuel_resource δ1 fs1 fs2 s2). *)
+  (*   { rewrite -Hsamedoms map_imap_dom_eq dom_gset_to_gmap //. *)
+  (*     { epose proof ls_fuel_dom as Hfueldom. intros ρ' Hin. *)
+  (*       destruct Hfuelsval as (?&?&?&?&?&Hdom_le). *)
+  (*       destruct (decide (ρ' ∈ live_roles _ δ1)). *)
+  (*       - apply elem_of_difference. *)
+  (*         split; [set_solver -Hnewdom Hsamedoms Hdom_le|]. *)
+  (*         intros [? Habs]%elem_of_difference. *)
+  (*         destruct (decide (ρ' = ρ)). *)
+  (*         + simplify_eq. apply not_elem_of_dom in Habs. *)
+  (*           rewrite -> Habs in *. simpl in *. eauto. *)
+  (*         + apply Habs. *)
+  (*           assert (ρ' ∈ dom fs1 ∖ {[ρ]}); set_solver -Hnewdom Hsamedoms. *)
+  (*       - apply elem_of_difference. *)
+  (*         split; [apply elem_of_union; right; set_unfold; naive_solver| *)
+  (*                  set_unfold; naive_solver]. } *)
+  (*     intros ρ0??. destruct (decide (ρ0 ∈ dom $ ls_fuel δ1)); [|done]. *)
+  (*     apply elem_of_dom. rewrite ls_same_doms. SS. } *)
+  (*   (* iExists {| *) *)
+  (*   (*   ls_under := s2; *) *)
+  (*   (*   ls_fuel :=  _; *) *)
+  (*   (*   ls_fuel_dom := Hfueldom; *) *)
+  (*   (*   ls_mapping := _; *) *)
+  (*   (*   ls_same_doms := Hsamedoms; *) *)
+  (*   (* |}.  *) *)
+  (*   iExists (build_LS_ext s2 _ Hfueldom (<[ζ:=dom fs2]> (ls_tmap δ1 (LM := LM))) _ _ (LM := LM)). *)
+  (*   iExists (Take_step ρ ζ). *)
+  (*   (* Unshelve. *) *)
+  (*   iMod (update_has_fuels _ fs1 fs2 with "Hfuel Hafuel Hamapping") as "(Hafuel & Hfuel & Hmapping)". *)
+  (*   { set_solver. } *)
+  (*   { unfold valid_new_fuelmap in Hfuelsval. *)
+  (*     destruct Hfuelsval as (_&_&?&?& Hfs2_inf&Hfs2_sup). *)
+  (*     apply elem_of_equiv_empty_L => ρ0 Hin. *)
+  (*     apply elem_of_intersection in Hin as [Hin1 Hin2]. *)
+  (*     apply elem_of_difference in Hin1 as [Hin11 Hin12]. *)
+  (*     assert (ρ0 ∈ live_roles _ s2 ∖ live_roles _ s1) *)
+  (*            by set_solver -Hsamedoms Hnewdom. *)
+  (*     assert (ρ0 ∈ fr1) by set_solver -Hsamedoms Hnewdom. *)
+  (*     assert (ρ0 ∈ FR) by set_solver -Hsamedoms Hnewdom. *)
+  (*     assert (ρ0 ∉ dom (ls_fuel δ1)) by set_solver -Hsamedoms Hnewdom. *)
+  (*     done. } *)
+  (*   iMod (update_model s2 with "Hamod Hmod") as "[Hamod Hmod]". *)
 
 
-    (* iMod (update_free_roles (live_roles M s2 ∖ live_roles M s1) *)
-    (*        with "HFR Hfr1") as "[HFR Hfr2]"; [set_solver|]. *)
-    pose proof (proj1 (subseteq_disjoint_union_L _ _) HfrFR) as [FR' [FR_EQ DISJ']].
-    iMod (update_free_roles_strong fr1 (fr1 ∖ (live_roles _ s2 ∖ live_roles _ s1) ∪ fr_stash) FR' with "[HFR] [Hfr1]") as "[HFR Hfr2]"; auto.
-    { apply disjoint_union_l. split; [set_solver| ].
-      eapply disjoint_subseteq.
-      { apply _. } (* TODO: why is it needed explicitly? *)
-      { apply Hstash_own. }
-      { eapply subseteq_proper; [reflexivity|..].
-        { apply leibniz_equiv_iff, FR_EQ. }
-        set_solver. }
-      rewrite -ls_same_doms in HFR.
-      clear -HFR Hxdom.
-      eapply disjoint_subseteq; [apply _| |reflexivity|].
-      2: { symmetry. apply disjoint_intersection. apply leibniz_equiv_iff, HFR. }
-      apply elem_of_subseteq. intros ? ?%Hxdom.
-      eapply elem_of_dom_2; eauto. }
-    { by rewrite FR_EQ. }
+  (*   (* iMod (update_free_roles (live_roles M s2 ∖ live_roles M s1) *) *)
+  (*   (*        with "HFR Hfr1") as "[HFR Hfr2]"; [set_solver|]. *) *)
+  (*   pose proof (proj1 (subseteq_disjoint_union_L _ _) HfrFR) as [FR' [FR_EQ DISJ']]. *)
+  (*   iMod (update_free_roles_strong fr1 (fr1 ∖ (live_roles _ s2 ∖ live_roles _ s1) ∪ fr_stash) FR' with "[HFR] [Hfr1]") as "[HFR Hfr2]"; auto. *)
+  (*   { apply disjoint_union_l. split; [set_solver| ]. *)
+  (*     eapply disjoint_subseteq. *)
+  (*     { apply _. } (* TODO: why is it needed explicitly? *) *)
+  (*     { apply Hstash_own. } *)
+  (*     { eapply subseteq_proper; [reflexivity|..]. *)
+  (*       { apply leibniz_equiv_iff, FR_EQ. } *)
+  (*       set_solver. } *)
+  (*     rewrite -ls_same_doms in HFR. *)
+  (*     clear -HFR Hxdom. *)
+  (*     eapply disjoint_subseteq; [apply _| |reflexivity|]. *)
+  (*     2: { symmetry. apply disjoint_intersection. apply leibniz_equiv_iff, HFR. } *)
+  (*     apply elem_of_subseteq. intros ? ?%Hxdom. *)
+  (*     eapply elem_of_dom_2; eauto. } *)
+  (*   { by rewrite FR_EQ. } *)
     
-    assert (maps_inverse_match new_mapping (<[ζ:=dom fs2]> (ls_tmap δ1 (LM := LM)))) as MATCH.
-    { intros ρ' ζ'. simpl. rewrite map_lookup_imap.
-      rewrite lookup_gset_to_gmap //=.
-      destruct (decide (ρ' ∈ (dom (ls_fuel δ1) ∪ dom fs2) ∖ (dom fs1 ∖ dom fs2))) as [Hin|Hnotin].
-      - rewrite option_guard_True //=. destruct (decide (ρ' ∈ dom (ls_fuel δ1))).
-        + destruct (decide (ζ' = ζ)) as [->|Hneq].
-          * rewrite lookup_insert. split.
-            { eexists; split =>//. apply elem_of_difference in Hin as [? Hin].
-              apply not_elem_of_difference in Hin as [?|?]; [|done].
-              set_solver -Hsamedoms Hnewdom Hfueldom. }
-            { intros (?&?&?). simplify_eq. apply Hxdom.
-              destruct Hfuelsval as (?&?&?&?&?). by_contradiction.
-              assert (ρ' ∈ live_roles M s2 ∖ live_roles M δ1) by set_solver -Hsamedoms Hnewdom Hfueldom.
-              assert (ρ' ∈ fr1) by set_solver -Hsamedoms Hnewdom Hfueldom.
-              assert (ρ' ∈ (fr1 ∪ FR')) by set_solver -Hsamedoms Hnewdom Hfueldom.
-              assert (ρ' ∉ dom $ ls_fuel δ1) by set_solver -Hsamedoms Hnewdom Hfueldom.
-              done. }
-          * rewrite lookup_insert_ne //.
-            apply ls_mapping_tmap_corr. 
-        + split.
-          * intros Htid. simplify_eq. rewrite lookup_insert. eexists; split=>//.
-            set_solver -Hsamedoms Hnewdom Hfueldom.
-          * assert (ρ' ∈ dom fs2) by set_solver -Hsamedoms Hnewdom Hfueldom. intros Hm. by_contradiction.
-            rewrite lookup_insert_ne in Hm; last congruence.
-            apply ls_mapping_tmap_corr in Hm. 
-            apply elem_of_dom_2 in Hm. rewrite ls_same_doms // in Hm.
-      - destruct Hfuelsval as (?&?&?&?&Hinf&?). rewrite option_guard_False //=. split; first done.
-        destruct (decide (ζ' = ζ)) as [->|Hneq].
-        { rewrite lookup_insert //. intros (?&?&?). simplify_eq. set_solver -Hsamedoms Hnewdom Hfueldom. }
-        rewrite lookup_insert_ne //.        
-        intros Habs%ls_mapping_tmap_corr.
+  (*   assert (maps_inverse_match new_mapping (<[ζ:=dom fs2]> (ls_tmap δ1 (LM := LM)))) as MATCH. *)
+  (*   { intros ρ' ζ'. simpl. rewrite map_lookup_imap. *)
+  (*     rewrite lookup_gset_to_gmap //=. *)
+  (*     destruct (decide (ρ' ∈ (dom (ls_fuel δ1) ∪ dom fs2) ∖ (dom fs1 ∖ dom fs2))) as [Hin|Hnotin]. *)
+  (*     - rewrite option_guard_True //=. destruct (decide (ρ' ∈ dom (ls_fuel δ1))). *)
+  (*       + destruct (decide (ζ' = ζ)) as [->|Hneq]. *)
+  (*         * rewrite lookup_insert. split. *)
+  (*           { eexists; split =>//. apply elem_of_difference in Hin as [? Hin]. *)
+  (*             apply not_elem_of_difference in Hin as [?|?]; [|done]. *)
+  (*             set_solver -Hsamedoms Hnewdom Hfueldom. } *)
+  (*           { intros (?&?&?). simplify_eq. apply Hxdom. *)
+  (*             destruct Hfuelsval as (?&?&?&?&?). by_contradiction. *)
+  (*             assert (ρ' ∈ live_roles M s2 ∖ live_roles M δ1) by set_solver -Hsamedoms Hnewdom Hfueldom. *)
+  (*             assert (ρ' ∈ fr1) by set_solver -Hsamedoms Hnewdom Hfueldom. *)
+  (*             assert (ρ' ∈ (fr1 ∪ FR')) by set_solver -Hsamedoms Hnewdom Hfueldom. *)
+  (*             assert (ρ' ∉ dom $ ls_fuel δ1) by set_solver -Hsamedoms Hnewdom Hfueldom. *)
+  (*             done. } *)
+  (*         * rewrite lookup_insert_ne //. *)
+  (*           apply ls_mapping_tmap_corr.  *)
+  (*       + split. *)
+  (*         * intros Htid. simplify_eq. rewrite lookup_insert. eexists; split=>//. *)
+  (*           set_solver -Hsamedoms Hnewdom Hfueldom. *)
+  (*         * assert (ρ' ∈ dom fs2) by set_solver -Hsamedoms Hnewdom Hfueldom. intros Hm. by_contradiction. *)
+  (*           rewrite lookup_insert_ne in Hm; last congruence. *)
+  (*           apply ls_mapping_tmap_corr in Hm.  *)
+  (*           apply elem_of_dom_2 in Hm. rewrite ls_same_doms // in Hm. *)
+  (*     - destruct Hfuelsval as (?&?&?&?&Hinf&?). rewrite option_guard_False //=. split; first done. *)
+  (*       destruct (decide (ζ' = ζ)) as [->|Hneq]. *)
+  (*       { rewrite lookup_insert //. intros (?&?&?). simplify_eq. set_solver -Hsamedoms Hnewdom Hfueldom. } *)
+  (*       rewrite lookup_insert_ne //.         *)
+  (*       intros Habs%ls_mapping_tmap_corr. *)
 
-        apply not_elem_of_difference in Hnotin as [Hnin|Hin].
-        + apply elem_of_dom_2 in Habs. rewrite ls_same_doms in Habs. set_solver -Hsamedoms Hnewdom Hfueldom.
-        + apply elem_of_difference in Hin as [Hin Hnin].
-          apply Hxdom in Hin. congruence. }
+  (*       apply not_elem_of_difference in Hnotin as [Hnin|Hin]. *)
+  (*       + apply elem_of_dom_2 in Habs. rewrite ls_same_doms in Habs. set_solver -Hsamedoms Hnewdom Hfueldom. *)
+  (*       + apply elem_of_difference in Hin as [Hin Hnin]. *)
+  (*         apply Hxdom in Hin. congruence. } *)
 
-    iModIntro.
-    iSplit.
-    { iSplit; first done. iPureIntro.
-      destruct Hfuelsval as (Hlim&Hzombie&Hinfs1m&Hnewlim&Hdec&Hinf&Hsup).
-      constructor =>//; split.
-      - constructor; simpl.
-        { rewrite build_LS_ext_spec_st. by rewrite Heq //. }
-        split; first by apply Hxdom; set_solver.
-        split.
-        { intros ? ? Hdom Hmd. inversion Hmd; clear Hmd; simplify_eq.
-          + symmetry in Hsametid. rewrite -> Hxdom in Hsametid. simpl.
-            unfold update_fuel_resource, fuel_apply.
-            rewrite build_LS_ext_spec_fuel. 
-            rewrite map_lookup_imap lookup_gset_to_gmap.
-            destruct (decide (ρ' ∈ live_roles M s2 ∪ dom fs2)) as [Hin|Hin].
-            * rewrite option_guard_True //=.
-              { destruct (decide (ρ' ∈ dom fs2)) as [Hin2|Hin2].
-                ** rewrite Hfuel; last set_solver.
-                   apply Hdec; [congruence|set_solver -Hsamedoms Hnewdom Hdom].
-                ** exfalso. set_solver -Hsamedoms Hnewdom Hdom. }
-              apply elem_of_difference; split;
-                [set_solver -Hsamedoms Hnewdom Hdom|].
-              apply not_elem_of_difference; right.
-              apply elem_of_union in Hin as [|]; [|done].
-              destruct (decide (ρ' = ρ)); simplify_eq.
-              apply Hinf; set_solver -Hsamedoms Hnewdom Hdom.
-            * rewrite option_guard_False //=.
-              ** assert (ρ' ∈ dom fs2); set_solver -Hsamedoms Hnewdom Hdom.
-              ** apply not_elem_of_difference; right; set_solver -Hsamedoms Hnewdom Hdom.
-          + simpl in *. unfold update_fuel_resource, fuel_apply.
-            rewrite build_LS_ext_spec_fuel. 
-            rewrite map_lookup_imap lookup_gset_to_gmap.
+  (*   iModIntro. *)
+  (*   iSplit. *)
+  (*   { iSplit; first done. iPureIntro. *)
+  (*     destruct Hfuelsval as (Hlim&Hzombie&Hinfs1m&Hnewlim&Hdec&Hinf&Hsup). *)
+  (*     constructor =>//; split. *)
+  (*     - constructor; simpl. *)
+  (*       { rewrite build_LS_ext_spec_st. by rewrite Heq //. } *)
+  (*       split; first by apply Hxdom; set_solver. *)
+  (*       split. *)
+  (*       { intros ? ? Hdom Hmd. inversion Hmd; clear Hmd; simplify_eq. *)
+  (*         + symmetry in Hsametid. rewrite -> Hxdom in Hsametid. simpl. *)
+  (*           unfold update_fuel_resource, fuel_apply. *)
+  (*           rewrite build_LS_ext_spec_fuel.  *)
+  (*           rewrite map_lookup_imap lookup_gset_to_gmap. *)
+  (*           destruct (decide (ρ' ∈ live_roles M s2 ∪ dom fs2)) as [Hin|Hin]. *)
+  (*           * rewrite option_guard_True //=. *)
+  (*             { destruct (decide (ρ' ∈ dom fs2)) as [Hin2|Hin2]. *)
+  (*               ** rewrite Hfuel; last set_solver. *)
+  (*                  apply Hdec; [congruence|set_solver -Hsamedoms Hnewdom Hdom]. *)
+  (*               ** exfalso. set_solver -Hsamedoms Hnewdom Hdom. } *)
+  (*             apply elem_of_difference; split; *)
+  (*               [set_solver -Hsamedoms Hnewdom Hdom|]. *)
+  (*             apply not_elem_of_difference; right. *)
+  (*             apply elem_of_union in Hin as [|]; [|done]. *)
+  (*             destruct (decide (ρ' = ρ)); simplify_eq. *)
+  (*             apply Hinf; set_solver -Hsamedoms Hnewdom Hdom. *)
+  (*           * rewrite option_guard_False //=. *)
+  (*             ** assert (ρ' ∈ dom fs2); set_solver -Hsamedoms Hnewdom Hdom. *)
+  (*             ** apply not_elem_of_difference; right; set_solver -Hsamedoms Hnewdom Hdom. *)
+  (*         + simpl in *. unfold update_fuel_resource, fuel_apply. *)
+  (*           rewrite build_LS_ext_spec_fuel.  *)
+  (*           rewrite map_lookup_imap lookup_gset_to_gmap. *)
 
-            erewrite build_LS_ext_spec_mapping in Hneqtid, Hissome.
-            2, 3: by eauto.
-            destruct (decide (ρ' ∈ (dom (ls_fuel δ1) ∪ dom fs2) ∖ (dom fs1 ∖ dom fs2))) as [Hin|Hin].
-            * rewrite map_lookup_imap lookup_gset_to_gmap option_guard_True //= decide_True //= in Hneqtid.
-            * apply not_elem_of_difference in Hin as [?|Hin];
-                [set_solver -Hsamedoms Hnewdom Hdom|].
-              apply elem_of_difference in Hin as [??].
-              rewrite map_lookup_imap lookup_gset_to_gmap /= option_guard_False /= in Hissome;
-                [inversion Hissome; congruence|set_solver -Hsamedoms Hnewdom Hdom].
-          + simpl in *. rewrite Hfuel; last set_solver -Hsamedoms Hnewdom Hdom.
-            unfold update_fuel_resource, fuel_apply.
-            rewrite build_LS_ext_spec_fuel in Hnotdead, Hdom. 
-            rewrite Hnewdom in Hnotdead.
-            rewrite build_LS_ext_spec_fuel. 
-            rewrite map_lookup_imap lookup_gset_to_gmap option_guard_True //=.
-            assert (ρ' ∈ dom fs2) by (set_solver -Hsamedoms Hnewdom Hdom).
-            rewrite decide_True; [| done]. 
-            apply Hzombie =>//; [| set_solver]. 
-            rewrite build_LS_ext_spec_st in Hnotalive. 
-            set_solver -Hsamedoms Hnewdom Hdom. 
-    }
-        split.
-        + intros ? Hin ?.
-          rewrite build_LS_ext_spec_fuel. 
-          simplify_eq; simpl.
-          unfold update_fuel_resource, fuel_apply.
-          rewrite map_lookup_imap lookup_gset_to_gmap.
-          destruct (decide (ρ' ∈ (dom (ls_fuel δ1) ∪ dom fs2) ∖ (dom fs1 ∖ dom fs2))) as [Hlive|Hlive].
-          * rewrite option_guard_True //=.
-            apply elem_of_difference in Hlive as [Hin1 Hnin].
-            apply not_elem_of_difference in Hnin.
-            destruct (decide (ρ' ∈ dom fs2)) as [Hin2|Hin2].
-            ** destruct (decide (ρ' ∈ live_roles _ δ1)); left.
-               *** destruct (decide (ρ' ∈ dom fs1)).
-                   { rewrite Hfuel //. apply oleq_oless, Hdec; [congruence|set_solver -Hsamedoms Hnewdom]. }
-                   { exfalso. set_solver -Hsamedoms Hnewdom. }
-               *** assert (ρ' ∉ live_roles _ s2).
-                   { by_contradiction. assert (ρ' ∈ fr1); [eapply elem_of_subseteq; eauto; set_solver -Hsamedoms Hnewdom|].
-                     assert (ρ' ∈ (fr1 ∪ FR')); [eapply elem_of_subseteq; eauto; set_solver -Hsamedoms Hnewdom|set_solver -Hsamedoms Hnewdom]. }
-                   assert (ρ' ∈ dom fs1) by set_solver -Hsamedoms Hnewdom.
-                   rewrite Hfuel //. apply oleq_oless, Hdec; [congruence|set_solver -Hsamedoms Hnewdom].
-            ** left. rewrite elem_of_dom in Hin. destruct Hin as [? ->]. simpl;lia.
-          * right; split.
-            ** eapply not_elem_of_weaken; [|by apply map_imap_dom_inclusion; rewrite dom_gset_to_gmap].
-               rewrite dom_gset_to_gmap //.
-            ** apply not_elem_of_difference in Hlive as [?|Hlive]; [set_solver -Hsamedoms Hnewdom|].
-               apply elem_of_difference in Hlive as [? Habs].
-               exfalso. apply Habs. set_solver -Hsamedoms Hnewdom Hfueldom.
-        +
-          rewrite build_LS_ext_spec_fuel build_LS_ext_spec_st.          
-          split.
-          { intros Hlive.
+  (*           erewrite build_LS_ext_spec_mapping in Hneqtid, Hissome. *)
+  (*           2, 3: by eauto. *)
+  (*           destruct (decide (ρ' ∈ (dom (ls_fuel δ1) ∪ dom fs2) ∖ (dom fs1 ∖ dom fs2))) as [Hin|Hin]. *)
+  (*           * rewrite map_lookup_imap lookup_gset_to_gmap option_guard_True //= decide_True //= in Hneqtid. *)
+  (*           * apply not_elem_of_difference in Hin as [?|Hin]; *)
+  (*               [set_solver -Hsamedoms Hnewdom Hdom|]. *)
+  (*             apply elem_of_difference in Hin as [??]. *)
+  (*             rewrite map_lookup_imap lookup_gset_to_gmap /= option_guard_False /= in Hissome; *)
+  (*               [inversion Hissome; congruence|set_solver -Hsamedoms Hnewdom Hdom]. *)
+  (*         + simpl in *. rewrite Hfuel; last set_solver -Hsamedoms Hnewdom Hdom. *)
+  (*           unfold update_fuel_resource, fuel_apply. *)
+  (*           rewrite build_LS_ext_spec_fuel in Hnotdead, Hdom.  *)
+  (*           rewrite Hnewdom in Hnotdead. *)
+  (*           rewrite build_LS_ext_spec_fuel.  *)
+  (*           rewrite map_lookup_imap lookup_gset_to_gmap option_guard_True //=. *)
+  (*           assert (ρ' ∈ dom fs2) by (set_solver -Hsamedoms Hnewdom Hdom). *)
+  (*           rewrite decide_True; [| done].  *)
+  (*           apply Hzombie =>//; [| set_solver].  *)
+  (*           rewrite build_LS_ext_spec_st in Hnotalive.  *)
+  (*           set_solver -Hsamedoms Hnewdom Hdom.  *)
+  (*   } *)
+  (*       split. *)
+  (*       + intros ? Hin ?. *)
+  (*         rewrite build_LS_ext_spec_fuel.  *)
+  (*         simplify_eq; simpl. *)
+  (*         unfold update_fuel_resource, fuel_apply. *)
+  (*         rewrite map_lookup_imap lookup_gset_to_gmap. *)
+  (*         destruct (decide (ρ' ∈ (dom (ls_fuel δ1) ∪ dom fs2) ∖ (dom fs1 ∖ dom fs2))) as [Hlive|Hlive]. *)
+  (*         * rewrite option_guard_True //=. *)
+  (*           apply elem_of_difference in Hlive as [Hin1 Hnin]. *)
+  (*           apply not_elem_of_difference in Hnin. *)
+  (*           destruct (decide (ρ' ∈ dom fs2)) as [Hin2|Hin2]. *)
+  (*           ** destruct (decide (ρ' ∈ live_roles _ δ1)); left. *)
+  (*              *** destruct (decide (ρ' ∈ dom fs1)). *)
+  (*                  { rewrite Hfuel //. apply oleq_oless, Hdec; [congruence|set_solver -Hsamedoms Hnewdom]. } *)
+  (*                  { exfalso. set_solver -Hsamedoms Hnewdom. } *)
+  (*              *** assert (ρ' ∉ live_roles _ s2). *)
+  (*                  { by_contradiction. assert (ρ' ∈ fr1); [eapply elem_of_subseteq; eauto; set_solver -Hsamedoms Hnewdom|]. *)
+  (*                    assert (ρ' ∈ (fr1 ∪ FR')); [eapply elem_of_subseteq; eauto; set_solver -Hsamedoms Hnewdom|set_solver -Hsamedoms Hnewdom]. } *)
+  (*                  assert (ρ' ∈ dom fs1) by set_solver -Hsamedoms Hnewdom. *)
+  (*                  rewrite Hfuel //. apply oleq_oless, Hdec; [congruence|set_solver -Hsamedoms Hnewdom]. *)
+  (*           ** left. rewrite elem_of_dom in Hin. destruct Hin as [? ->]. simpl;lia. *)
+  (*         * right; split. *)
+  (*           ** eapply not_elem_of_weaken; [|by apply map_imap_dom_inclusion; rewrite dom_gset_to_gmap]. *)
+  (*              rewrite dom_gset_to_gmap //. *)
+  (*           ** apply not_elem_of_difference in Hlive as [?|Hlive]; [set_solver -Hsamedoms Hnewdom|]. *)
+  (*              apply elem_of_difference in Hlive as [? Habs]. *)
+  (*              exfalso. apply Habs. set_solver -Hsamedoms Hnewdom Hfueldom. *)
+  (*       + *)
+  (*         rewrite build_LS_ext_spec_fuel build_LS_ext_spec_st.           *)
+  (*         split. *)
+  (*         { intros Hlive. *)
             
-            unfold update_fuel_resource, fuel_apply.
-          destruct (decide (ρ ∈ (dom (ls_fuel δ1) ∪ dom fs2) ∖ (dom fs1 ∖ dom fs2))) as [Hin|Hnin].
-          - rewrite map_lookup_imap lookup_gset_to_gmap option_guard_True //=. 
-            rewrite decide_True; [by apply Hlim |set_solver -Hsamedoms Hnewdom Hfueldom].
-          - exfalso; apply not_elem_of_difference in Hnin as [Hnin|Hnin].
-            + assert (ρ ∉ live_roles _ δ1).
-              eapply not_elem_of_weaken => //.
-              { epose proof ls_fuel_dom. set_solver -Hsamedoms Hnewdom Hfueldom. }
-              assert (ρ ∈ dom fs2) by set_solver -Hsamedoms Hnewdom Hfueldom. set_solver -Hsamedoms Hnewdom Hfueldom.
-            + apply elem_of_difference in Hnin as [? Hnin].
-              apply not_elem_of_dom in Hnin. rewrite Hnin /= in Hlim.
-              by apply Hlim. }
-          split.
-          { intros ρ'. unfold update_fuel_resource, fuel_apply => Hin.
-            rewrite map_imap_dom_eq in Hin; last first.
-            { intros ρ0 _ Hin'. destruct (decide (ρ0 ∈ dom fs2)); [by apply elem_of_dom|].
-              rewrite dom_gset_to_gmap elem_of_difference in Hin'.
-              destruct Hin' as [Hin' ?]. apply elem_of_union in Hin' as [?|?]; [by apply elem_of_dom|done]. }
-            rewrite dom_gset_to_gmap in Hin. rewrite map_lookup_imap lookup_gset_to_gmap option_guard_True /=; last set_solver -Hsamedoms Hnewdom Hfueldom.
-            assert (ρ' ∈ dom fs2) by set_solver -Hsamedoms Hnewdom Hfueldom. rewrite decide_True //. apply Hnewlim. apply elem_of_difference; split =>//.
-            intros contra%Hxdom%elem_of_dom_2. rewrite ls_same_doms in contra. simplify_eq. set_solver -Hsamedoms Hnewdom Hfueldom. }
-          intros ρ0 Hin.
-          assert (ρ0 ∉ live_roles _ δ1).
-          { eapply not_elem_of_weaken; last apply ls_fuel_dom. set_solver -Hsamedoms Hnewdom Hfueldom. }
-          apply elem_of_difference in Hin as [Hin1 Hnin].
-          assert (ρ0 ∈ live_roles _ s2).
-          { by_contradiction.
-            assert (ρ0 ∈ dom fs2).
-            { unfold update_fuel_resource, fuel_apply in Hin1.
-              eapply elem_of_subseteq in Hin1; last apply map_imap_dom_inclusion.
-              rewrite dom_gset_to_gmap in Hin1. set_solver -Hsamedoms Hnewdom Hfueldom. }
-            exfalso. assert (Hinabs: ρ0 ∈ dom fs1) by set_solver -Hsamedoms Hnewdom Hfueldom.
-            apply not_elem_of_dom in Hnin. rewrite Hfuel // in Hnin.
-            apply elem_of_dom in Hinabs. rewrite Hnin in Hinabs. simpl in Hinabs.
-            by inversion Hinabs. }
-          set_solver -Hsamedoms Hnewdom Hfueldom.
-      - eapply tids_smaller_model_step; eauto.
-        erewrite build_LS_ext_spec_mapping; eauto. }
+  (*           unfold update_fuel_resource, fuel_apply. *)
+  (*         destruct (decide (ρ ∈ (dom (ls_fuel δ1) ∪ dom fs2) ∖ (dom fs1 ∖ dom fs2))) as [Hin|Hnin]. *)
+  (*         - rewrite map_lookup_imap lookup_gset_to_gmap option_guard_True //=.  *)
+  (*           rewrite decide_True; [by apply Hlim |set_solver -Hsamedoms Hnewdom Hfueldom]. *)
+  (*         - exfalso; apply not_elem_of_difference in Hnin as [Hnin|Hnin]. *)
+  (*           + assert (ρ ∉ live_roles _ δ1). *)
+  (*             eapply not_elem_of_weaken => //. *)
+  (*             { epose proof ls_fuel_dom. set_solver -Hsamedoms Hnewdom Hfueldom. } *)
+  (*             assert (ρ ∈ dom fs2) by set_solver -Hsamedoms Hnewdom Hfueldom. set_solver -Hsamedoms Hnewdom Hfueldom. *)
+  (*           + apply elem_of_difference in Hnin as [? Hnin]. *)
+  (*             apply not_elem_of_dom in Hnin. rewrite Hnin /= in Hlim. *)
+  (*             by apply Hlim. } *)
+  (*         split. *)
+  (*         { intros ρ'. unfold update_fuel_resource, fuel_apply => Hin. *)
+  (*           rewrite map_imap_dom_eq in Hin; last first. *)
+  (*           { intros ρ0 _ Hin'. destruct (decide (ρ0 ∈ dom fs2)); [by apply elem_of_dom|]. *)
+  (*             rewrite dom_gset_to_gmap elem_of_difference in Hin'. *)
+  (*             destruct Hin' as [Hin' ?]. apply elem_of_union in Hin' as [?|?]; [by apply elem_of_dom|done]. } *)
+  (*           rewrite dom_gset_to_gmap in Hin. rewrite map_lookup_imap lookup_gset_to_gmap option_guard_True /=; last set_solver -Hsamedoms Hnewdom Hfueldom. *)
+  (*           assert (ρ' ∈ dom fs2) by set_solver -Hsamedoms Hnewdom Hfueldom. rewrite decide_True //. apply Hnewlim. apply elem_of_difference; split =>//. *)
+  (*           intros contra%Hxdom%elem_of_dom_2. rewrite ls_same_doms in contra. simplify_eq. set_solver -Hsamedoms Hnewdom Hfueldom. } *)
+  (*         intros ρ0 Hin. *)
+  (*         assert (ρ0 ∉ live_roles _ δ1). *)
+  (*         { eapply not_elem_of_weaken; last apply ls_fuel_dom. set_solver -Hsamedoms Hnewdom Hfueldom. } *)
+  (*         apply elem_of_difference in Hin as [Hin1 Hnin]. *)
+  (*         assert (ρ0 ∈ live_roles _ s2). *)
+  (*         { by_contradiction. *)
+  (*           assert (ρ0 ∈ dom fs2). *)
+  (*           { unfold update_fuel_resource, fuel_apply in Hin1. *)
+  (*             eapply elem_of_subseteq in Hin1; last apply map_imap_dom_inclusion. *)
+  (*             rewrite dom_gset_to_gmap in Hin1. set_solver -Hsamedoms Hnewdom Hfueldom. } *)
+  (*           exfalso. assert (Hinabs: ρ0 ∈ dom fs1) by set_solver -Hsamedoms Hnewdom Hfueldom. *)
+  (*           apply not_elem_of_dom in Hnin. rewrite Hfuel // in Hnin. *)
+  (*           apply elem_of_dom in Hinabs. rewrite Hnin in Hinabs. simpl in Hinabs. *)
+  (*           by inversion Hinabs. } *)
+  (*         set_solver -Hsamedoms Hnewdom Hfueldom. *)
+  (*     - eapply tids_smaller_model_step; eauto. *)
+  (*       erewrite build_LS_ext_spec_mapping; eauto. } *)
 
-    iFrame "Hfuel Hmod Hfr2".
+  (*   iFrame "Hfuel Hmod Hfr2". *)
 
-    iExists _.
-    rewrite build_LS_ext_spec_st build_LS_ext_spec_fuel build_LS_ext_spec_tmap. 
-    iFrame. all: eauto. (* TODO: find source... *)
-    iPureIntro; split.
+  (*   iExists _. *)
+  (*   rewrite build_LS_ext_spec_st build_LS_ext_spec_fuel build_LS_ext_spec_tmap.  *)
+  (*   iFrame. all: eauto. (* TODO: find source... *) *)
+  (*   iPureIntro; split. *)
         
-    { intros. eapply tids_restrict_model_step; eauto.
-      eapply ls_mapping_tmap_corr; eauto.
-      apply Hxdom. apply Hfuelsval. }
+  (*   { intros. eapply tids_restrict_model_step; eauto. *)
+  (*     eapply ls_mapping_tmap_corr; eauto. *)
+  (*     apply Hxdom. apply Hfuelsval. } *)
 
-    { simpl. rewrite /update_fuel_resource /fuel_apply.
-      rewrite map_imap_dom_eq ?dom_gset_to_gmap.
-      + apply elem_of_equiv_empty_L. intros ρ' [Hin1 Hin2]%elem_of_intersection.
+  (*   { simpl. rewrite /update_fuel_resource /fuel_apply. *)
+  (*     rewrite map_imap_dom_eq ?dom_gset_to_gmap. *)
+  (*     + apply elem_of_equiv_empty_L. intros ρ' [Hin1 Hin2]%elem_of_intersection. *)
 
-        (* TODO: problems with elem_of_proper *)
-        assert (fr1 ∖ (live_roles M s2 ∖ live_roles M s1) ∪ fr_stash ∪ FR' ≡ FR ∖ (live_roles M s2 ∖ live_roles M s1) ∪ fr_stash ∪ FR' ∩ (live_roles M s2 ∖ live_roles M s1)) as ALT.
-        { set_solver. }
-        rewrite ALT in Hin1. 
+  (*       (* TODO: problems with elem_of_proper *) *)
+  (*       assert (fr1 ∖ (live_roles M s2 ∖ live_roles M s1) ∪ fr_stash ∪ FR' ≡ FR ∖ (live_roles M s2 ∖ live_roles M s1) ∪ fr_stash ∪ FR' ∩ (live_roles M s2 ∖ live_roles M s1)) as ALT. *)
+  (*       { set_solver. } *)
+  (*       rewrite ALT in Hin1.  *)
 
-        apply elem_of_union in Hin1 as [[Hin1 | Hin1] %elem_of_union | Hin1].
-        2, 3: set_solver. 
-        apply elem_of_difference in Hin1 as [Hin11 Hin12].
-        apply not_elem_of_difference in Hin12.
-        apply elem_of_difference in Hin2 as [Hin21 Hin22].
-        apply not_elem_of_difference in Hin22.
-        assert (ρ' ∉ dom $ ls_fuel δ1) by set_solver -Hsamedoms Hnewdom Hfueldom.
-        assert (ρ' ∈ dom fs2) by set_solver -Hsamedoms Hnewdom Hfueldom.
-        destruct Hin12 as [Hin12|Hin12]; last by (epose proof ls_fuel_dom; set_solver -Hsamedoms Hnewdom Hfueldom).
-        destruct Hfuelsval as (?&?&?&?&?&?).
-        assert (ρ' ∉ dom fs1); last set_solver -Hsamedoms Hnewdom Hfueldom.
-        intros contra. pose proof (Hfuel _ contra) as Habs. apply elem_of_dom in contra as [? contra].
-        rewrite contra in Habs. apply elem_of_dom_2 in Habs. done. 
-    + intros ρ' _ Hin. destruct (decide (ρ' ∈ dom fs2)) as [Hin'|].
-      * apply elem_of_dom in Hin' as [? ->]. done.
-      * assert (ρ' ∈ dom (ls_fuel δ1)) as Hin' by set_solver -Hsamedoms Hnewdom Hfueldom. apply elem_of_dom in Hin' as [? ->]. done. }
+  (*       apply elem_of_union in Hin1 as [[Hin1 | Hin1] %elem_of_union | Hin1]. *)
+  (*       2, 3: set_solver.  *)
+  (*       apply elem_of_difference in Hin1 as [Hin11 Hin12]. *)
+  (*       apply not_elem_of_difference in Hin12. *)
+  (*       apply elem_of_difference in Hin2 as [Hin21 Hin22]. *)
+  (*       apply not_elem_of_difference in Hin22. *)
+  (*       assert (ρ' ∉ dom $ ls_fuel δ1) by set_solver -Hsamedoms Hnewdom Hfueldom. *)
+  (*       assert (ρ' ∈ dom fs2) by set_solver -Hsamedoms Hnewdom Hfueldom. *)
+  (*       destruct Hin12 as [Hin12|Hin12]; last by (epose proof ls_fuel_dom; set_solver -Hsamedoms Hnewdom Hfueldom). *)
+  (*       destruct Hfuelsval as (?&?&?&?&?&?). *)
+  (*       assert (ρ' ∉ dom fs1); last set_solver -Hsamedoms Hnewdom Hfueldom. *)
+  (*       intros contra. pose proof (Hfuel _ contra) as Habs. apply elem_of_dom in contra as [? contra]. *)
+  (*       rewrite contra in Habs. apply elem_of_dom_2 in Habs. done.  *)
+  (*   + intros ρ' _ Hin. destruct (decide (ρ' ∈ dom fs2)) as [Hin'|]. *)
+  (*     * apply elem_of_dom in Hin' as [? ->]. done. *)
+  (*     * assert (ρ' ∈ dom (ls_fuel δ1)) as Hin' by set_solver -Hsamedoms Hnewdom Hfueldom. apply elem_of_dom in Hin' as [? ->]. done. } *)
 
-    Unshelve. all: eauto.
-    - admit.
-    - admit. 
-  Admitted. 
+  (*   Unshelve. all: eauto. *)
+  (*   - admit. *)
+  (*   - admit.  *)
+  (* Admitted.  *)
 
 
 End ActualOwnershipImpl.
