fairness/heap_lang/em_lm.v
@@ -29,6 +29,41 @@ Definition lm_cfg_init (σ: cfg heap_lang) :=
 Definition lm_is_init_st `{LM: LiveModel heap_lang M} σ s := 
   lm_cfg_init σ /\ lm_model_init s (LM := LM). 
 
+Definition tids_restrict `{M: FairModel} `{Countable (locale Λ)}
+  (c: cfg Λ) (tmap: gmap (locale Λ) (gset (fmrole M))): Prop :=
+  forall ζ, ζ ∉ locales_of_list c.1 → tmap !! ζ = None.
+
+(* TODO: unify with existing locales_of_list_from_locale_from, 
+   remove restriction for heap_lang *)
+Lemma locales_of_list_from_locale_from' tp0 tp1 ζ:
+  ζ ∈ locales_of_list_from tp0 tp1 (Λ := heap_lang) ->
+  is_Some (from_locale_from tp0 tp1 ζ).
+Proof.
+  clear -tp0 tp1 ζ.
+  revert tp0; induction tp1 as [|e1 tp1 IH]; intros tp0.
+  { simpl. intros H. inversion H. }
+  simpl.
+  rewrite /locales_of_list_from /=. intros.
+  destruct (decide (locale_of tp0 e1 = ζ)); simplify_eq; first set_solver.
+  apply elem_of_cons in H as [?| ?]; [done| ].
+  set_solver.
+Qed.
+
+Lemma tids_restrict_smaller `{LM:LiveModel heap_lang M} (σ: cfg heap_lang) (δ: lm_ls LM):
+  tids_restrict σ (ls_tmap δ) -> tids_smaller σ.1 δ.
+Proof.
+  rewrite /tids_smaller /tids_restrict. 
+  intros. apply locales_of_list_from_locale_from'.
+  destruct (decide (ζ ∈ locales_of_list σ.1)); [done| ].
+  specialize (H _ n).
+  eapply (ls_mapping_tmap_corr (LM := LM)) in H0 as [R [? ?]].
+  congruence. 
+Qed. 
+
+Definition em_lm_msi `{LM:LiveModel heap_lang M} `{!fairnessGS LM Σ}
+  (c: cfg heap_lang) (δ: mstate LM): iProp Σ :=
+  model_state_interp δ ∗ ⌜ tids_restrict c (ls_tmap δ (LM := LM)) ⌝. 
+
 (* TODO: how to make 'heap..' instantiations less wordy? *)
 (* TODO: how to avoid different instances of EqDec and Cnt? *)
 Lemma init_fairnessGS_LM Σ `{hPre: @fairnessGpreS heap_lang M LM Σ
@@ -39,7 +74,7 @@ Lemma init_fairnessGS_LM Σ `{hPre: @fairnessGpreS heap_lang M LM Σ
   ⊢ (|==> ∃ fGS: fairnessGS LM Σ, (* TODO: what is a canonical way of doing it? *)
        (* ∀ `{hGS: @heapGS Σ _ (@LM_EM _ LM)}, *)
        (*   ⌜ hGS.(heap_fairnessGS) = fGS⌝ → *)
-      LM_init_resource s1 ∗ model_state_interp σ1 s1).
+      LM_init_resource s1 ∗ em_lm_msi σ1 s1).
 Proof.
   iIntros. 
   destruct INIT as [[??] [FUEL TMAP]]. destruct σ1 as [tp ?]. simpl in *. subst.
@@ -57,9 +92,10 @@ Proof.
               fairness_model_fuel_name := γfuel;
               fairness_model_free_roles_name := γfr;
             |}).
-
-  iSplitL "Hmodf Hfr Hfuelf Hmapf".
-  2: { unfold model_state_interp. simpl. iFrame. 
+  
+  iApply bi.sep_comm. rewrite /em_lm_msi. rewrite -bi.sep_assoc.  
+  iSplitR "Hmodf Hfr Hfuelf Hmapf".
+  1: { unfold model_state_interp. simpl. iFrame. 
        iExists _.
 
        iSplitL "Hfuela".
@@ -68,13 +104,18 @@ Proof.
 
        iSplitL "Hmapa"; first by rewrite TMAP /auth_mapping_is /= map_fmap_singleton //.
        iSplit; first done.
-       iSplit; iPureIntro. 
        (* - intros ρ tid. rewrite MAP.  *)
        (*   rewrite lookup_gset_to_gmap_Some. *)
        (*   setoid_rewrite lookup_singleton_Some. split; naive_solver. *)
-       - intros tid Hlocs. rewrite TMAP lookup_singleton_ne //.
-         compute in Hlocs. set_solver.
-       - rewrite FUEL. rewrite dom_gset_to_gmap. set_solver. }
+
+       (* - rewrite FUEL. rewrite dom_gset_to_gmap. set_solver. *)
+       iPureIntro. set_solver. 
+  }
+
+  iSplitR.
+  { iPureIntro. rewrite /tids_restrict.
+    intros tid Hlocs. rewrite TMAP lookup_singleton_ne //.
+    compute in Hlocs. set_solver. }    
 
   rewrite /LM_init_resource /has_fuels /=.
     
@@ -120,7 +161,7 @@ refine
 (* TODO: cannot directly specify these components *)
 Unshelve. 
 { exact (valid_evolution_step (LM := LM)). }
-2: { intros ? fG. exact (model_state_interp (LM := LM) (fG := fG)). } 
+2: { intros ? fG. exact (em_lm_msi (LM := LM) (fairnessGS0 := fG)). } 
 intros. iIntros. iMod (init_fairnessGS_LM _ s1 σ) as "[% [? X]]"; [done| ]. 
 iModIntro. iExists _. iFrame. 
 Defined. 
@@ -136,3 +177,53 @@ Global Instance LM_EM_fair `{LM: LiveModel heap_lang M}
                 `{hGS: @heapGS Σ LM (@LM_EM _ LM)}:
   fairnessGS LM Σ.
 Proof. apply hGS. Defined.
+
+Lemma tids_smaller_restrict_mapping `{M: FairModel}
+
+  (c1 c2: cfg heap_lang) δ1 δ2 (ζ: locale heap_lang)
+  (Hζs : tids_smaller c1.1 δ1)
+  (DOM12: ls_mapping δ2 ⊆ ls_mapping δ1)
+  (STEP: locale_step c1 (Some ζ) c2)
+  :
+  tids_smaller c2.1 δ2 (M := M).
+Proof.
+  unfold tids_smaller; simpl.
+  intros ρ ζ0 Hin.
+  destruct c1, c2.
+  eapply from_locale_step =>//.
+  rewrite /tids_smaller /= in Hζs. eapply Hζs.
+  eapply lookup_weaken; eauto. 
+Qed.
+
+Lemma tids_dom_restrict_mapping `{LM: LiveModel heap_lang M} 
+  (c1 c2: cfg heap_lang)
+  (tmap1 tmap2: gmap (locale heap_lang) (gset (fmrole M))) (ζ: locale heap_lang)
+  (Hstep : locale_step c1 (Some ζ) c2)
+  (Hlocssmall: tids_restrict c1 tmap1)
+  (TMAP2: exists S, tmap2 = <[ζ:=S]> (tmap1))
+  :
+  tids_restrict c2 tmap2.
+Proof.
+  intros ζ0 Hnotin.
+  destruct TMAP2 as [? ->]. 
+  destruct c1, c2. simpl in *. 
+  apply lookup_insert_None; split.
+  + apply Hlocssmall.
+    have Hle := locales_of_list_step_incl _ _ _ _ _ Hstep. simpl.
+    clear -Hnotin Hle. set_solver.
+  + intros <-. 
+    have ? := locales_of_list_step_incl _ _ _ _ _ Hstep. simpl.
+    (* clear Hfueldom Hsamedoms. *)
+    inversion Hstep. simplify_eq.
+    assert (locale_of t1 e1 ∈ locales_of_list (t1 ++ e1 :: t2));
+      last by eauto.
+    apply locales_of_list_from_locale_from.
+    rewrite from_locale_from_Some //. 
+    eapply prefixes_from_spec.
+    eexists _,_. by list_simplifier.
+Qed.
+  (* TODO: ?? *)
+    (* - rewrite Hnewdom /new_dom. apply elem_of_equiv_empty_L. intros ρ [Hin1 Hin2]%elem_of_intersection. *)
+    (*   assert (ρ ∈ dom (ls_fuel δ1)) *)
+    (*     by set_solver -Hnewdom Hsamedoms Hfueldom. *)
+    (*   set_solver -Hnewdom Hsamedoms Hfueldom. } *) 
