fairness/actual_resources_interface.v
@@ -2,25 +2,66 @@ From iris.algebra Require Import auth gmap gset excl.
 From iris.proofmode Require Import tactics.
 From trillium.fairness Require Import fairness fuel resources actual_resources heap_lang_defs em_lm pmp_lifting.
 
+
+(* TODO: move *)
+Section Utils.
+  Context `{Countable K, Countable V, EqDecision K}.
+  
+  Lemma maps_inverse_match_subseteq (m1 m2: gmap K V) (m1' m2': gmap V (gset K))
+    (M1: maps_inverse_match m1 m1') (M2: maps_inverse_match m2 m2')
+    (SUB: dom m1' ⊆ dom m2')
+    (INCL: forall v S1 S2, m1' !! v = Some S1 -> m2' !! v = Some S2 -> S1 ⊆ S2):
+    m1 ⊆ m2.
+  Proof.
+    red in M1, M2. apply map_subseteq_spec. intros.
+    specialize (proj1 (M1 _ _) H1) as [? [L1 ?]]. 
+    apply M2.
+    specialize (SUB x (elem_of_dom_2 _ _ _ L1)).
+    apply elem_of_dom in SUB as [? ?].
+    eexists. split; eauto. set_solver.
+  Qed. 
+
+End Utils.
+
 Section ActualOwnershipInterface. 
   Context `{LM: LiveModel heap_lang M}.
-  (* Context `{Countable (locale Λ)}. *)
-  (* Context `{EqDecision (expr Λ)}. *)
   Context {Σ : gFunctors}.
   Context {fG: fairnessGS LM Σ}.
   Context`{invGS_gen HasNoLc Σ}. 
 
+  (* TODO: replace Definitions with Lets in pmp_lifting.v *)
   Lemma ActualOwnershipPartial:
     ⊢ PartialModelPredicates ∅ (EM := @LM_EM _ LM) (iLM := LM) (PMPP := ActualOwnershipPartialPre) (eGS := fG). 
   Proof.
     iIntros. iApply Build_PartialModelPredicates. iModIntro. repeat iSplitL.
-    - iIntros. iApply (actual_update_no_step_enough_fuel with "[$]"); set_solver.
-    - iIntros. iMod (actual_update_fork_split with "[$] [$]") as (?) "?"; eauto.
-    - iIntros "*". iIntros.
-      iApply (actual_update_step_still_alive with "[$] [$] [$] [$]"); eauto.
-    - iIntros. iApply (frag_free_roles_fuels_disj with "[$] [$] [$]").
-    - iIntros. iExists _. iFrame.
-      iIntros. do 2 iExists _. by iFrame.
+    - iIntros. rewrite /update_no_step_enough_fuel_def. 
+      iIntros "FUELS MSI". simpl in *.
+      iDestruct "MSI" as "[LM_MSI %TR]".
+      iDestruct (has_fuel_in with "FUELS LM_MSI") as %Hxdom; eauto.
+
+      iMod (actual_update_no_step_enough_fuel with "FUELS LM_MSI") as (?) "(%STEPM & FUELS & LM_MSI' & %TMAP')".
+      3: by apply empty_subseteq. 2: set_solver. 1: done. 
+      iModIntro. do 2 iExists _. rewrite /em_lm_msi. iFrame.
+      iPureIntro. split.
+      + remember (trace_last auxtr) as δ1. 
+        pose proof (tids_restrict_smaller _ _ TR) as SM.
+        repeat split; eauto.
+        * done.
+        * eapply tids_smaller_restrict_mapping; eauto.
+          erewrite (maps_inverse_match_uniq1 (ls_mapping δ2)).
+          3: { eapply (mim_fuel_helper _ ∅); eauto.
+               { set_solver. }
+               eapply ls_mapping_tmap_corr. }
+          { apply map_filter_subseteq. }
+          erewrite <- TMAP'. apply ls_mapping_tmap_corr.
+      + eapply tids_dom_restrict_mapping; eauto.
+    (* - iIntros. iMod (actual_update_fork_split with "[$] [$]") as (?) "?"; eauto. *)
+    (* - iIntros "*". iIntros. *)
+    (*   iApply (actual_update_step_still_alive with "[$] [$] [$] [$]"); eauto. *)
+    (* - iIntros. iApply (frag_free_roles_fuels_disj with "[$] [$] [$]"). *)
+    (* - iIntros. iExists _. iFrame. *)
+    (*   iIntros. do 2 iExists _. by iFrame. *)
   Defined.
+
 
 End ActualOwnershipInterface.  
